examples/AKE/AKE_proof.ec
@@ -187,6 +187,7 @@ module AKE(FA : Adv) = {
     init();
 
     while (i < qAgent) {
+      i = i + 1;
       ska = $sample_Sk;
       pka = gen_pk(ska);
       pks = pka :: pks;
@@ -405,6 +406,7 @@ module AKE_EexpRev(FA : Adv2) = {
     
     init();
     while (i < qAgent) {
+      i = i + 1;
       ska = $sample_Sk;
       pka = gen_pk(ska);
       pks = pka :: pks;
@@ -460,314 +462,37 @@ end section.
 
 (*{ Proof: Pr[ AKE : win ] <= eps + Pr[ AKE_EexpRev : win ] *)
 
-op esk_of_sidx (mStarted : (Sidx, Sdata) map) (i : Sidx) =
-  sd_esk(proj mStarted.[i]).
+section.
 
-op esks(mStarted : (Sidx, Sdata) map) : Esk set =
-  img sd_esk (frng mStarted).
+declare module A : Adv{ AKE, AKE_EexpRev }.
 
-op queried_esks(mH1 : ((Sk * Esk), Eexp)  map) : Esk set =
-  img snd (fdom mH1).
+axiom A_Lossless_choose : 
+  forall (O <: AKE_Oracles{A}),
+    islossless O.h1_a =>
+    islossless O.h2_a =>
+    islossless O.init1 =>
+    islossless O.init2 =>
+    islossless O.resp =>
+    islossless O.staticRev =>
+    islossless O.ephemeralRev =>
+    islossless O.sessionRev =>
+    islossless A(O).choose.
 
-(* Introduce bad flags for collision events and split mStarted.
-   Use accessor functions instead of pattern matching in computeKey.
-   Strengthen if-condition such that all map lookups are guarded in sessionRev
-   and computeKey. *)
-module AKE_1(FA : Adv) = {
-  
-  var evs  : Event list               (* events for queries performed by adversary *)
-  var test : Sid option               (* session id of test session *)
-
-  var cH1, cH2 : int                  (* counters for queries *)
-
-  var mH1 : ((Sk * Esk), Eexp) map    (* map for h1 *)
-  var sH1 : (Sk * Esk) set            (* adversary queries for h1 *)
-
-  var mH2 : (Sstring, Key) map        (* map for h2 *)
-  var sH2 : Sstring set               (* adversary queries for h2 *)
-
-  var mSk        : (Agent, Sk) map    (* map for static secret keys *)
-  var mStarted   : (Sidx, Sdata) map  (* map of started sessions *)
-  var mCompleted : (Sidx, Epk)   map  (* additional data for completed sessions *)
-
-  var bad_esk_col : bool              (* esk collision with dom(mH1) *)
-    (* The esk sampled in init1/resp is already in dom(mH1). Since
-       dom(mH1) = sH1 u <earlier esks>, this corresponds to
-       esk-earlier-esk collisions and esk-earlier-h1_a collisions *)
-
-  var bad_esk_norev : bool            (* h1_a query without previous reveal *)
-  
-  fun init() : unit = {
-    evs = [];
-    test = None;
-    cH1 = 0;
-    cH2 = 0;
-    mH1 = Map.empty;
-    sH1 = FSet.empty;
-    mH2 = Map.empty;
-    sH2 = FSet.empty;
-    mSk = Map.empty;
-    mStarted = Map.empty;
-    mCompleted = Map.empty;
-    bad_esk_col = false;
-    bad_esk_norev = false;
-  }
-
-  module O : AKE_Oracles = {
-
-    fun h1(a : Sk, x : Esk) : Eexp = {
-      var e : Eexp;
-      e = $sample_Eexp;
-      if (!in_dom (a,x) mH1) {
-        mH1.[(a,x)] = e;
-      } 
-      return proj mH1.[(a,x)];
-    }
-
-    fun h1_a(a : Sk, x : Esk) : Eexp option = {
-      var r : Eexp option = None;
-      var xe : Eexp;
-      if (cH1 < qH1) {
-        cH1 = cH1 + 1;
-        if (any (lambda i, let sd = proj mStarted.[i] in
-                           sd_esk sd = x /\
-                           ! (mem (EphemeralRev (psid_of_sdata sd)) evs))
-                (fdom mStarted)) {
-          bad_esk_norev = true;
-        }
-        sH1 = add (a,x) sH1;
-        xe = h1(a,x);
-        r = Some(xe);
-      }
-      return r;
-    }
-
-    fun h2(sstring : Sstring) : Key = {
-      var ke : Key;
-      ke = $sample_Key;
-      if (!in_dom sstring mH2) {
-        mH2.[sstring] = ke;
-      }
-      return proj mH2.[sstring];
-    }
- 
-    fun h2_a(sstring : Sstring) : Key option = {
-      var r : Key option = None;
-      var ks : Key;
-      if (cH2 < qH2) {
-        cH2 = cH2 + 1;
-        sH2 = add sstring sH2;
-        ks = h2(sstring);
-        r = Some(ks);
-      }
-      return r;
-    }
-
-    fun init1(i : Sidx, A : Agent, B : Agent) : Epk option = {
-      var pX : Epk;
-      var x : Esk;
-      var x' : Eexp;
-      var r : Epk option = None; 
-      if (in_dom A mSk && in_dom B mSk && !in_dom i mStarted) {
-        x  = $sample_Esk;
-        if (mem x (queried_esks mH1)) bad_esk_col = true;
-        x' = h1(proj (mSk.[A]),x);
-        pX = gen_epk(x');
-        mStarted.[i] = (A,B,x,x',init);
-        r = Some(pX);
-        evs = Start(psid_of_sdata(proj mStarted.[i]))::evs;
-      }
-      return r;
-    }
-
-    fun resp(i : Sidx, B : Agent, A : Agent, X : Epk) : Epk option = {
-      var y : Esk;
-      var y' : Eexp;
-      var pY : Epk;
-      var r : Epk option = None; 
-      if (in_dom A mSk && in_dom B mSk && !in_dom i mStarted && !in_dom i mCompleted) {
-        y  = $sample_Esk;
-        if (mem y (queried_esks mH1)) bad_esk_col = true;
-        y' = h1(proj (mSk.[B]),y);
-        pY = gen_epk(y');
-        mStarted.[i] = (B,A,y,y',resp);
-        mCompleted.[i] = X;
-        r = Some(pY);
-        evs = Accept(sid_of_sdata (proj mStarted.[i]) X)::evs;
-      }
-      return r;
-    }
-
-    fun init2(i : Sidx, Y : Epk) : unit = {
-      if (!in_dom i mCompleted && in_dom i mStarted) {
-        mCompleted.[i] = Y;
-        evs = Accept(sid_of_sdata(proj mStarted.[i]) Y)::evs;
-      }
-    }
-
-    fun staticRev(A : Agent) : Sk option = {
-      var r : Sk option = None;
-      if (in_dom A mSk) {
-        r = mSk.[A];
-        evs = StaticRev(A)::evs;
-      }
-      return r;
-    }
-
-    fun ephemeralRev(i : Sidx) : Esk option = {
-      var r : Esk option = None;
-      if (in_dom i mStarted) {
-        r = Some(sd_esk(proj mStarted.[i]));
-        evs = EphemeralRev(psid_of_sdata(proj mStarted.[i]))::evs;
-      }
-      return r;
-    }
-
-    fun computeKey(i : Sidx) : Key option = {
-      var r : Key option = None;
-      var sd : Sdata;
-      var k : Key;
-      if (in_dom i mCompleted && in_dom i mStarted) {
-        sd = proj mStarted.[i];
-        k = h2(gen_sstring (sd_eexp sd) (proj mSk.[sd_actor sd])
-                           (sd_peer sd) (proj mCompleted.[i])
-                           (sd_role sd));
-        r = Some k;
-      }
-      return r;
-    }
-
-    fun sessionRev(i : Sidx) : Key option = {
-      var r : Key option = None;
-      if (in_dom i mCompleted && in_dom i mStarted) {
-        evs = SessionRev(sid_of_sdata(proj mStarted.[i]) (proj mCompleted.[i]))::evs;
-        r = computeKey(i);
-      }
-      return r;
-    }
-  }
-  
-  module A = FA(O)
-
-  fun main() : bool = {
-    var b : bool = def;
-    var pks : Pk list = [];
-    var t_idx : Sidx = def;
-    var key : Key = def;
-    var keyo : Key option = def;
-    var b' : bool = def;
-    var i : int = 0;
-    var ska : Sk = def;
-    var pka : Pk = def;
-
-    init();
-
-    while (i < qAgent) {
-      ska = $sample_Sk;
-      pka = gen_pk(ska);
-      pks = pka :: pks;
-      mSk.[pka] = ska;
-    } 
-
-    t_idx = A.choose(pks);
-    b = ${0,1};
-    if (mStarted.[t_idx] <> None && mCompleted.[t_idx] <> None) {
-      test = Some (sid_of_sdata (proj mStarted.[t_idx]) (proj mCompleted.[t_idx]));
-        (* the if-condition implies "mem (Accept (proj O.test)) O.evs" *)
-      if (b) {
-        keyo = O.computeKey(t_idx);
-      } else {
-        key  = $sample_Key;
-        keyo = Some key;
-      }
-      b' = A.guess(keyo);
-    }
-    return (b = b');
-  }
-}.
-
-lemma Eq_AKE_AKE_1_O_h1(A <: Adv{AKE, AKE_1}):
-  equiv[ AKE(A).O.h1 ~ AKE_1(A).O.h1 :
-         (AKE.mH1{1} = AKE_1.mH1{2} /\ ={x,a})
-         ==> (AKE.mH1{1} = AKE_1.mH1{2} /\ ={res}) ].
-proof strict.
-  by fun; eqobs_in.
-qed.
-
-lemma Eq_AKE_AKE_1_O_h2(A <: Adv{AKE, AKE_1}):
-  equiv[ AKE(A).O.h2 ~ AKE_1(A).O.h2 :
-         (AKE.mH2{1} = AKE_1.mH2{2} /\ ={sstring})
-         ==> (AKE.mH2{1} = AKE_1.mH2{2} /\ ={res}) ].
-proof strict.
-  by fun; eqobs_in.
-qed.
-   
-lemma Eq_AKE_AKE_1(A <: Adv{AKE, AKE_1}):
-  equiv[ AKE(A).main ~ AKE_1(A).main : true ==>
-            (res /\ test_fresh AKE.test AKE.evs){1}
-         => (res /\ test_fresh AKE_1.test AKE_1.evs){2}].
-proof strict.
-  fun.
-  eqobs_in
-    (AKE.mSk{1}        = AKE_1.mSk{2} /\
-     AKE.cH1{1}        = AKE_1.cH1{2} /\
-     AKE.cH2{1}        = AKE_1.cH2{2} /\
-     AKE.mH1{1}        = AKE_1.mH1{2} /\
-     AKE.sH1{1}        = AKE_1.sH1{2} /\
-     AKE.mH2{1}        = AKE_1.mH2{2} /\
-     AKE.sH2{1}        = AKE_1.sH2{2} /\
-     AKE.mStarted{1}   = AKE_1.mStarted{2} /\
-     AKE.mCompleted{1} = AKE_1.mCompleted{2} /\
-     AKE.evs{1}        = AKE_1.evs{2} /\
-     AKE.test{1}       = AKE_1.test{2})
-    true :
-    (={b,pks,t_idx,key,keyo,b',i,ska,pka} /\
-     AKE.mSk{1}        = AKE_1.mSk{2} /\
-     AKE.cH1{1}        = AKE_1.cH1{2} /\
-     AKE.cH2{1}        = AKE_1.cH2{2} /\
-     AKE.mH1{1}        = AKE_1.mH1{2} /\
-     AKE.sH1{1}        = AKE_1.sH1{2} /\
-     AKE.mH2{1}        = AKE_1.mH2{2} /\
-     AKE.sH2{1}        = AKE_1.sH2{2} /\
-     AKE.mStarted{1}   = AKE_1.mStarted{2} /\
-     AKE.mCompleted{1} = AKE_1.mCompleted{2} /\
-     AKE.evs{1}        = AKE_1.evs{2} /\
-     AKE.test{1}       = AKE_1.test{2}).
-    (* computeKey *)
-    fun.
-    sp.
-    if; [ by smt | | skip; by smt].
-    wp.
-    call (Eq_AKE_AKE_1_O_h2 A).
-    by wp; skip; smt.
-
-    (* resp *)
-    fun.
-    sp.
-    if; [ by smt | | skip; by smt].
-    wp.
-    call (Eq_AKE_AKE_1_O_h1 A).
-    by wp; rnd; wp; skip; smt.
-
-    (* init1 *)
-    fun.
-    sp.
-    if; [ by smt | | skip; by smt].
-    wp.
-    call (Eq_AKE_AKE_1_O_h1 A).
-    by wp; rnd; wp; skip; smt.
-
-    (* h1_a *)
-    fun.
-    sp.
-    if; [ smt | | skip; smt].
-    wp.
-    call (Eq_AKE_AKE_1_O_h1 A).
-    by wp; skip; smt.
-qed.
+axiom A_Lossless_guess : 
+  forall (O <: AKE_Oracles{A}),
+    islossless O.h1_a =>
+    islossless O.h2_a =>
+    islossless O.init1 =>
+    islossless O.init2 =>
+    islossless O.resp =>
+    islossless O.staticRev =>
+    islossless O.ephemeralRev =>
+    islossless O.sessionRev =>
+    islossless A(O).guess.
 
 (* Split mStarted into three maps. *)
-module AKE_2(FA : Adv) = {
+local
+module AKE_1(FA : Adv) = {
   
   var evs  : Event list               (* events for queries performed by adversary *)
   var test : Sid option               (* session id of test session *)
@@ -786,13 +511,6 @@ module AKE_2(FA : Adv) = {
   var mStarted   : (Sidx, Sdata2) map (* map of started sessions *)
   var mCompleted : (Sidx, Epk)   map  (* additional data for completed sessions *)
 
-  var bad_esk_col : bool              (* esk collision with dom(mH1) *)
-    (* The esk sampled in init1/resp is already in dom(mH1). Since
-       dom(mH1) = sH1 u <earlier esks>, this corresponds to
-       esk-earlier-esk collisions and esk-earlier-h1_a collisions *)
-
-  var bad_esk_norev : bool            (* h1_a query without previous reveal *)
-
   fun init() : unit = {
     evs = [];
     test = None;
@@ -807,8 +525,6 @@ module AKE_2(FA : Adv) = {
     mEexp = Map.empty;
     mStarted = Map.empty;
     mCompleted = Map.empty;
-    bad_esk_col = false;
-    bad_esk_norev = false;
   }
 
   module O : AKE_Oracles = {
@@ -827,11 +543,6 @@ module AKE_2(FA : Adv) = {
       var xe : Eexp;
       if (cH1 < qH1) {
         cH1 = cH1 + 1;
-        if (any (lambda i, proj mEsk.[i] = x /\
-                           ! (mem (EphemeralRev (compute_psid mStarted mEexp i)) evs))
-                (fdom mStarted)) {
-          bad_esk_norev = true;
-        }
         sH1 = add (a,x) sH1;
         xe = h1(a,x);
         r = Some(xe);
@@ -867,7 +578,6 @@ module AKE_2(FA : Adv) = {
       if (in_dom A mSk && in_dom B mSk && !in_dom i mStarted) {
         x = $sample_Esk;
         mEsk.[i] = x;
-        if (mem x (queried_esks mH1)) bad_esk_col = true;
         mEexp.[i] = h1(proj (mSk.[A]),x);
         pX = gen_epk(proj mEexp.[i]);
         mStarted.[i] = (A,B,init);
@@ -884,7 +594,6 @@ module AKE_2(FA : Adv) = {
       if (in_dom A mSk && in_dom B mSk && !in_dom i mStarted && !in_dom i mCompleted) {
         y  = $sample_Esk;
         mEsk.[i] = y;
-        if (mem y (queried_esks mH1)) bad_esk_col = true;
         mEexp.[i] = h1(proj (mSk.[B]),y);
         pY = gen_epk(proj mEexp.[i]);
         mStarted.[i] = (B,A,resp);
@@ -959,6 +668,7 @@ module AKE_2(FA : Adv) = {
 
     init();
     while (i < qAgent) {
+      i = i + 1;
       ska = $sample_Sk;
       pka = gen_pk(ska);
       pks = pka :: pks;
@@ -984,23 +694,7 @@ module AKE_2(FA : Adv) = {
 
 (*{ Definitions required for relational invariant between AKE_1 and AKE_2 *)
 
-(* we don't use the predicate because we cannot prevent automatic unfolding
-pred eq_map_split_pred
-                 (mStarted1 : (Sidx, Sdata)  map) 
-                 (mStarted2 : (Sidx, Sdata2) map) 
-                 (mEsk      : (Sidx, Esk)    map)
-                 (mEexp     : (Sidx, Eexp)   map)
-   =    dom mStarted1 = dom mStarted2 /\ dom mStarted2 = dom mEsk
-     /\ dom mStarted2 = dom mEexp /\
-     (forall (i : Sidx) (sd1 : Sdata) (A B : Agent) (r : Role),
-        in_dom i mStarted1 =>
-        sd_actor (proj mStarted1.[i]) = sd2_actor (proj mStarted2.[i]) /\
-        sd_peer  (proj mStarted1.[i]) = sd2_peer  (proj mStarted2.[i]) /\
-        sd_role  (proj mStarted1.[i]) = sd2_role  (proj mStarted2.[i]) /\
-        sd_esk   (proj mStarted1.[i]) = proj mEsk.[i] /\
-        sd_eexp  (proj mStarted1.[i]) = proj mEexp.[i]).
-*)
-
+(* we don't use the predicate because we cannot prevent automatic unfolding *)
 op eq_map_split : (Sidx, Sdata)  map ->
                   (Sidx, Sdata2) map ->
                   (Sidx, Esk)    map ->
@@ -1078,139 +772,98 @@ proof strict.
   by rewrite eq_map_split_def; smt.
 qed.
 
-lemma eq_map_split_5(mStarted1  : (Sidx, Sdata)  map)
-                    (mStarted2  : (Sidx, Sdata2) map)
-                    (mEsk       : (Sidx, Esk)    map) 
-                    (mEexp      : (Sidx, Eexp)   map)
-                    (evs : Event list)
-                    (x : Esk):
-     eq_map_split mStarted1 mStarted2 mEsk mEexp
-  =>   any (lambda i, let sd = proj mStarted1.[i] in
-                      sd_esk sd = x /\
-                      ! (mem (EphemeralRev (psid_of_sdata sd)) evs))
-           (fdom mStarted1)
-     = any (lambda i, proj mEsk.[i] = x /\
-                      ! (mem (EphemeralRev (compute_psid mStarted2 mEexp i)) evs))
-            (fdom mStarted2).
-proof strict.
-  rewrite eq_map_split_def /psid_of_sdata /compute_psid !any_def /fdom /fdom rw_eq_iff.
-  cut Fin1: ISet.Finite.finite (dom mStarted1). smt.
-    (* FIXME: make Sidx finite type 0 .. qsessions or axiomatize the condition *)
-  cut Fin2: ISet.Finite.finite (dom mStarted2). smt.
-  progress.
-  exists x0.
-  cut ->: mem x0 ((ISet.Finite.toFSet (dom mStarted2))) = ISet.mem x0 (dom mStarted2); first smt.
-  generalize H3;
-    cut ->:   mem x0 ((ISet.Finite.toFSet (dom mStarted1)))
-            = ISet.mem x0 (dom mStarted1); first smt;
-    intros=> H3.
-  smt.
-  exists x0.
-  cut ->:   mem x0 ((ISet.Finite.toFSet (dom mStarted1)))
-          = ISet.mem x0 (dom mStarted1); first smt.
-  generalize H3;
-    cut ->:   mem x0 ((ISet.Finite.toFSet (dom mStarted2)))
-            = ISet.mem x0 (dom mStarted2); first smt;
-    intros=> H3.
-  smt.
-qed.
-
 (*} end: Definitions required for relational invariant between AKE_1 and AKE_2 *)
 
 (*{ First handle oracles that are unaffected by changes *)
 
-lemma Eq_AKE_1_AKE_2_O_h1(A <: Adv{AKE, AKE_1}):
-  equiv[ AKE_1(A).O.h1 ~ AKE_2(A).O.h1 :
-         (AKE_1.mH1{1} = AKE_2.mH1{2} /\ ={x,a})
-         ==> (AKE_1.mH1{1} = AKE_2.mH1{2} /\ ={res}) ].
+local
+lemma Eq_AKE_AKE_1_O_h1:
+  equiv[ AKE(A).O.h1 ~ AKE_1(A).O.h1 :
+         (AKE.mH1{1} = AKE_1.mH1{2} /\ ={x,a})
+         ==> (AKE.mH1{1} = AKE_1.mH1{2} /\ ={res}) ].
 proof strict.
   by fun; eqobs_in.
 qed.
 
-lemma Eq_AKE_1_AKE_2_O_h2(A <: Adv{AKE, AKE_1}):
-  equiv[ AKE_1(A).O.h2 ~ AKE_2(A).O.h2 :
-         (AKE_1.mH2{1} = AKE_2.mH2{2} /\ ={sstring})
-         ==> (AKE_1.mH2{1} = AKE_2.mH2{2} /\ ={res}) ].
+local
+lemma Eq_AKE_AKE_1_O_h2:
+  equiv[ AKE(A).O.h2 ~ AKE_1(A).O.h2 :
+         (AKE.mH2{1} = AKE_1.mH2{2} /\ ={sstring})
+         ==> (AKE.mH2{1} = AKE_1.mH2{2} /\ ={res}) ].
 proof strict.
   by fun; eqobs_in.
 qed.
   
-lemma Eq_AKE_1_AKE_2_O_h2_a(A <: Adv{AKE, AKE_1}):
-  equiv[ AKE_1(A).O.h2_a ~ AKE_2(A).O.h2_a :
+local
+lemma Eq_AKE_AKE_1_O_h2_a:
+  equiv[ AKE(A).O.h2_a ~ AKE_1(A).O.h2_a :
          ( ={sstring} /\
-           AKE_1.evs{1}         = AKE_2.evs{2} /\
-           AKE_1.test{1}        = AKE_2.test{2} /\
-           AKE_1.cH1{1}         = AKE_2.cH1{2} /\
-           AKE_1.cH2{1}         = AKE_2.cH2{2} /\
-           AKE_1.mH1{1}         = AKE_2.mH1{2} /\
-           AKE_1.sH1{1}         = AKE_2.sH1{2} /\
-           AKE_1.mH2{1}         = AKE_2.mH2{2} /\
-           AKE_1.sH2{1}         = AKE_2.sH2{2} /\
-           AKE_1.mSk{1}         = AKE_2.mSk{2} /\
-           AKE_1.mCompleted{1}  = AKE_2.mCompleted{2} /\
-           AKE_1.bad_esk_col{1} = AKE_2.bad_esk_col{2} /\
-           AKE_1.bad_esk_norev{1} = AKE_2.bad_esk_norev{2} /\
-           eq_map_split AKE_1.mStarted{1} AKE_2.mStarted{2}
-                        AKE_2.mEsk{2} AKE_2.mEexp{2})
+           AKE.evs{1}         = AKE_1.evs{2} /\
+           AKE.test{1}        = AKE_1.test{2} /\
+           AKE.cH1{1}         = AKE_1.cH1{2} /\
+           AKE.cH2{1}         = AKE_1.cH2{2} /\
+           AKE.mH1{1}         = AKE_1.mH1{2} /\
+           AKE.sH1{1}         = AKE_1.sH1{2} /\
+           AKE.mH2{1}         = AKE_1.mH2{2} /\
+           AKE.sH2{1}         = AKE_1.sH2{2} /\
+           AKE.mSk{1}         = AKE_1.mSk{2} /\
+           AKE.mCompleted{1}  = AKE_1.mCompleted{2} /\
+           eq_map_split AKE.mStarted{1} AKE_1.mStarted{2}
+                        AKE_1.mEsk{2} AKE_1.mEexp{2})
          ==>
          ( ={res} /\
-           AKE_1.evs{1}         = AKE_2.evs{2} /\
-           AKE_1.test{1}        = AKE_2.test{2} /\
-           AKE_1.cH1{1}         = AKE_2.cH1{2} /\
-           AKE_1.cH2{1}         = AKE_2.cH2{2} /\
-           AKE_1.mH1{1}         = AKE_2.mH1{2} /\
-           AKE_1.sH1{1}         = AKE_2.sH1{2} /\
-           AKE_1.mH2{1}         = AKE_2.mH2{2} /\
-           AKE_1.sH2{1}         = AKE_2.sH2{2} /\
-           AKE_1.mSk{1}         = AKE_2.mSk{2} /\
-           AKE_1.mCompleted{1}  = AKE_2.mCompleted{2} /\
-           AKE_1.bad_esk_col{1} = AKE_2.bad_esk_col{2} /\
-           AKE_1.bad_esk_norev{1} = AKE_2.bad_esk_norev{2} /\
-           eq_map_split AKE_1.mStarted{1} AKE_2.mStarted{2}
-                        AKE_2.mEsk{2} AKE_2.mEexp{2}) ].
+           AKE.evs{1}         = AKE_1.evs{2} /\
+           AKE.test{1}        = AKE_1.test{2} /\
+           AKE.cH1{1}         = AKE_1.cH1{2} /\
+           AKE.cH2{1}         = AKE_1.cH2{2} /\
+           AKE.mH1{1}         = AKE_1.mH1{2} /\
+           AKE.sH1{1}         = AKE_1.sH1{2} /\
+           AKE.mH2{1}         = AKE_1.mH2{2} /\
+           AKE.sH2{1}         = AKE_1.sH2{2} /\
+           AKE.mSk{1}         = AKE_1.mSk{2} /\
+           AKE.mCompleted{1}  = AKE_1.mCompleted{2} /\
+           eq_map_split AKE.mStarted{1} AKE_1.mStarted{2}
+                        AKE_1.mEsk{2} AKE_1.mEexp{2}) ].
 proof strict.
   fun.
   sp.
   if; [ by smt | | by skip; smt ].
   wp.
-  call (Eq_AKE_1_AKE_2_O_h2 A).
+  call (Eq_AKE_AKE_1_O_h2).
   wp.
   skip; smt.
 qed.
 
-lemma Eq_AKE_1_AKE_2_O_staticRev(A <: Adv{AKE, AKE_1}):
-  equiv[ AKE_1(A).O.staticRev ~ AKE_2(A).O.staticRev :
+local
+lemma Eq_AKE_AKE_1_O_staticRev:
+  equiv[ AKE(A).O.staticRev ~ AKE_1(A).O.staticRev :
          ( ={A} /\
-           AKE_1.evs{1}         = AKE_2.evs{2} /\
-           AKE_1.test{1}        = AKE_2.test{2} /\
-           AKE_1.cH1{1}         = AKE_2.cH1{2} /\
-           AKE_1.cH2{1}         = AKE_2.cH2{2} /\
-           AKE_1.mH1{1}         = AKE_2.mH1{2} /\
-           AKE_1.sH1{1}         = AKE_2.sH1{2} /\
-           AKE_1.mH2{1}         = AKE_2.mH2{2} /\
-           AKE_1.sH2{1}         = AKE_2.sH2{2} /\
-           AKE_1.mSk{1}         = AKE_2.mSk{2} /\
-           AKE_1.mCompleted{1}  = AKE_2.mCompleted{2} /\
-           AKE_1.bad_esk_col{1} = AKE_2.bad_esk_col{2} /\
-           AKE_1.bad_esk_norev{1} = AKE_2.bad_esk_norev{2} /\
-           eq_map_split AKE_1.mStarted{1} AKE_2.mStarted{2}
-                        AKE_2.mEsk{2} AKE_2.mEexp{2})
+           AKE.evs{1}         = AKE_1.evs{2} /\
+           AKE.test{1}        = AKE_1.test{2} /\
+           AKE.cH1{1}         = AKE_1.cH1{2} /\
+           AKE.cH2{1}         = AKE_1.cH2{2} /\
+           AKE.mH1{1}         = AKE_1.mH1{2} /\
+           AKE.sH1{1}         = AKE_1.sH1{2} /\
+           AKE.mH2{1}         = AKE_1.mH2{2} /\
+           AKE.sH2{1}         = AKE_1.sH2{2} /\
+           AKE.mSk{1}         = AKE_1.mSk{2} /\
+           AKE.mCompleted{1}  = AKE_1.mCompleted{2} /\
+           eq_map_split AKE.mStarted{1} AKE_1.mStarted{2}
+                        AKE_1.mEsk{2} AKE_1.mEexp{2})
          ==>
          ( ={res} /\
-           AKE_1.evs{1}         = AKE_2.evs{2} /\
-           AKE_1.test{1}        = AKE_2.test{2} /\
-           AKE_1.cH1{1}         = AKE_2.cH1{2} /\
-           AKE_1.cH2{1}         = AKE_2.cH2{2} /\
-           AKE_1.mH1{1}         = AKE_2.mH1{2} /\
-           AKE_1.sH1{1}         = AKE_2.sH1{2} /\
-           AKE_1.mH2{1}         = AKE_2.mH2{2} /\
-           AKE_1.sH2{1}         = AKE_2.sH2{2} /\
-           AKE_1.mSk{1}         = AKE_2.mSk{2} /\
-           AKE_1.mCompleted{1}  = AKE_2.mCompleted{2} /\
-           AKE_1.bad_esk_col{1} = AKE_2.bad_esk_col{2} /\
-           AKE_1.bad_esk_norev{1} = AKE_2.bad_esk_norev{2} /\
-           eq_map_split AKE_1.mStarted{1} AKE_2.mStarted{2}
-                        AKE_2.mEsk{2} AKE_2.mEexp{2}) ].
+           AKE.evs{1}         = AKE_1.evs{2} /\
+           AKE.test{1}        = AKE_1.test{2} /\
+           AKE.cH1{1}         = AKE_1.cH1{2} /\
+           AKE.cH2{1}         = AKE_1.cH2{2} /\
+           AKE.mH1{1}         = AKE_1.mH1{2} /\
+           AKE.sH1{1}         = AKE_1.sH1{2} /\
+           AKE.mH2{1}         = AKE_1.mH2{2} /\
+           AKE.sH2{1}         = AKE_1.sH2{2} /\
+           AKE.mSk{1}         = AKE_1.mSk{2} /\
+           AKE.mCompleted{1}  = AKE_1.mCompleted{2} /\
+           eq_map_split AKE.mStarted{1} AKE_1.mStarted{2}
+                        AKE_1.mEsk{2} AKE_1.mEexp{2}) ].
 proof strict.
   fun; wp; skip; smt.
 qed.
@@ -1219,78 +872,72 @@ qed.
 
 (*{ Then handle oracles that only read the modified maps. *)
 
-lemma Eq_AKE_1_AKE_2_O_init2(A <: Adv{AKE, AKE_1}):
-  equiv[ AKE_1(A).O.init2 ~ AKE_2(A).O.init2 :
+local
+lemma Eq_AKE_AKE_1_O_init2:
+  equiv[ AKE(A).O.init2 ~ AKE_1(A).O.init2 :
           ( ={i,Y} /\
-           AKE_1.evs{1}         = AKE_2.evs{2} /\
-           AKE_1.test{1}        = AKE_2.test{2} /\
-           AKE_1.cH1{1}         = AKE_2.cH1{2} /\
-           AKE_1.cH2{1}         = AKE_2.cH2{2} /\
-           AKE_1.mH1{1}         = AKE_2.mH1{2} /\
-           AKE_1.sH1{1}         = AKE_2.sH1{2} /\
-           AKE_1.mH2{1}         = AKE_2.mH2{2} /\
-           AKE_1.sH2{1}         = AKE_2.sH2{2} /\
-           AKE_1.mSk{1}         = AKE_2.mSk{2} /\
-           AKE_1.mCompleted{1}  = AKE_2.mCompleted{2} /\
-           AKE_1.bad_esk_col{1} = AKE_2.bad_esk_col{2} /\
-           AKE_1.bad_esk_norev{1} = AKE_2.bad_esk_norev{2} /\
-           eq_map_split AKE_1.mStarted{1} AKE_2.mStarted{2}
-                        AKE_2.mEsk{2} AKE_2.mEexp{2})
+           AKE.evs{1}         = AKE_1.evs{2} /\
+           AKE.test{1}        = AKE_1.test{2} /\
+           AKE.cH1{1}         = AKE_1.cH1{2} /\
+           AKE.cH2{1}         = AKE_1.cH2{2} /\
+           AKE.mH1{1}         = AKE_1.mH1{2} /\
+           AKE.sH1{1}         = AKE_1.sH1{2} /\
+           AKE.mH2{1}         = AKE_1.mH2{2} /\
+           AKE.sH2{1}         = AKE_1.sH2{2} /\
+           AKE.mSk{1}         = AKE_1.mSk{2} /\
+           AKE.mCompleted{1}  = AKE_1.mCompleted{2} /\
+           eq_map_split AKE.mStarted{1} AKE_1.mStarted{2}
+                        AKE_1.mEsk{2} AKE_1.mEexp{2})
          ==>
           ( ={res} /\
-           AKE_1.evs{1}         = AKE_2.evs{2} /\
-           AKE_1.test{1}        = AKE_2.test{2} /\
-           AKE_1.cH1{1}         = AKE_2.cH1{2} /\
-           AKE_1.cH2{1}         = AKE_2.cH2{2} /\
-           AKE_1.mH1{1}         = AKE_2.mH1{2} /\
-           AKE_1.sH1{1}         = AKE_2.sH1{2} /\
-           AKE_1.mH2{1}         = AKE_2.mH2{2} /\
-           AKE_1.sH2{1}         = AKE_2.sH2{2} /\
-           AKE_1.mSk{1}         = AKE_2.mSk{2} /\
-           AKE_1.mCompleted{1}  = AKE_2.mCompleted{2} /\
-           AKE_1.bad_esk_col{1} = AKE_2.bad_esk_col{2} /\
-           AKE_1.bad_esk_norev{1} = AKE_2.bad_esk_norev{2} /\
-           eq_map_split AKE_1.mStarted{1} AKE_2.mStarted{2}
-                        AKE_2.mEsk{2} AKE_2.mEexp{2}) ].
+           AKE.evs{1}         = AKE_1.evs{2} /\
+           AKE.test{1}        = AKE_1.test{2} /\
+           AKE.cH1{1}         = AKE_1.cH1{2} /\
+           AKE.cH2{1}         = AKE_1.cH2{2} /\
+           AKE.mH1{1}         = AKE_1.mH1{2} /\
+           AKE.sH1{1}         = AKE_1.sH1{2} /\
+           AKE.mH2{1}         = AKE_1.mH2{2} /\
+           AKE.sH2{1}         = AKE_1.sH2{2} /\
+           AKE.mSk{1}         = AKE_1.mSk{2} /\
+           AKE.mCompleted{1}  = AKE_1.mCompleted{2} /\
+           eq_map_split AKE.mStarted{1} AKE_1.mStarted{2}
+                        AKE_1.mEsk{2} AKE_1.mEexp{2}) ].
 proof strict.
   fun.
   if ; [ by smt | | by skip; smt ].
   by wp; skip; smt.
 qed.
 
-lemma Eq_AKE_1_AKE_2_O_ephemeralRev(A <: Adv{AKE, AKE_1}):
-  equiv[ AKE_1(A).O.ephemeralRev ~ AKE_2(A).O.ephemeralRev :
+local
+lemma Eq_AKE_AKE_1_O_ephemeralRev:
+  equiv[ AKE(A).O.ephemeralRev ~ AKE_1(A).O.ephemeralRev :
           ( ={i} /\
-           AKE_1.evs{1}         = AKE_2.evs{2} /\
-           AKE_1.test{1}        = AKE_2.test{2} /\
-           AKE_1.cH1{1}         = AKE_2.cH1{2} /\
-           AKE_1.cH2{1}         = AKE_2.cH2{2} /\
-           AKE_1.mH1{1}         = AKE_2.mH1{2} /\
-           AKE_1.sH1{1}         = AKE_2.sH1{2} /\
-           AKE_1.mH2{1}         = AKE_2.mH2{2} /\
-           AKE_1.sH2{1}         = AKE_2.sH2{2} /\
-           AKE_1.mSk{1}         = AKE_2.mSk{2} /\
-           AKE_1.mCompleted{1}  = AKE_2.mCompleted{2} /\
-           AKE_1.bad_esk_col{1} = AKE_2.bad_esk_col{2} /\
-           AKE_1.bad_esk_norev{1} = AKE_2.bad_esk_norev{2} /\
-           eq_map_split AKE_1.mStarted{1} AKE_2.mStarted{2}
-                        AKE_2.mEsk{2} AKE_2.mEexp{2})
+           AKE.evs{1}         = AKE_1.evs{2} /\
+           AKE.test{1}        = AKE_1.test{2} /\
+           AKE.cH1{1}         = AKE_1.cH1{2} /\
+           AKE.cH2{1}         = AKE_1.cH2{2} /\
+           AKE.mH1{1}         = AKE_1.mH1{2} /\
+           AKE.sH1{1}         = AKE_1.sH1{2} /\
+           AKE.mH2{1}         = AKE_1.mH2{2} /\
+           AKE.sH2{1}         = AKE_1.sH2{2} /\
+           AKE.mSk{1}         = AKE_1.mSk{2} /\
+           AKE.mCompleted{1}  = AKE_1.mCompleted{2} /\
+           eq_map_split AKE.mStarted{1} AKE_1.mStarted{2}
+                        AKE_1.mEsk{2} AKE_1.mEexp{2})
          ==>
           ( ={res} /\
-           AKE_1.evs{1}         = AKE_2.evs{2} /\
-           AKE_1.test{1}        = AKE_2.test{2} /\
-           AKE_1.cH1{1}         = AKE_2.cH1{2} /\
-           AKE_1.cH2{1}         = AKE_2.cH2{2} /\
-           AKE_1.mH1{1}         = AKE_2.mH1{2} /\
-           AKE_1.sH1{1}         = AKE_2.sH1{2} /\
-           AKE_1.mH2{1}         = AKE_2.mH2{2} /\
-           AKE_1.sH2{1}         = AKE_2.sH2{2} /\
-           AKE_1.mSk{1}         = AKE_2.mSk{2} /\
-           AKE_1.mCompleted{1}  = AKE_2.mCompleted{2} /\
-           AKE_1.bad_esk_col{1} = AKE_2.bad_esk_col{2} /\
-           AKE_1.bad_esk_norev{1} = AKE_2.bad_esk_norev{2} /\
-           eq_map_split AKE_1.mStarted{1} AKE_2.mStarted{2}
-                        AKE_2.mEsk{2} AKE_2.mEexp{2}) ].
+           AKE.evs{1}         = AKE_1.evs{2} /\
+           AKE.test{1}        = AKE_1.test{2} /\
+           AKE.cH1{1}         = AKE_1.cH1{2} /\
+           AKE.cH2{1}         = AKE_1.cH2{2} /\
+           AKE.mH1{1}         = AKE_1.mH1{2} /\
+           AKE.sH1{1}         = AKE_1.sH1{2} /\
+           AKE.mH2{1}         = AKE_1.mH2{2} /\
+           AKE.sH2{1}         = AKE_1.sH2{2} /\
+           AKE.mSk{1}         = AKE_1.mSk{2} /\
+           AKE.mCompleted{1}  = AKE_1.mCompleted{2} /\
+           eq_map_split AKE.mStarted{1} AKE_1.mStarted{2}
+                        AKE_1.mEsk{2} AKE_1.mEexp{2}) ].
 proof strict.
   fun.
   wp;  skip; intros &1 &2.
@@ -1298,523 +945,612 @@ proof strict.
   by progress; smt.
 qed.
 
-lemma Eq_AKE_1_AKE_2_O_computeKey(A <: Adv{AKE, AKE_1}):
-  equiv[ AKE_1(A).O.computeKey ~ AKE_2(A).O.computeKey :
+local
+lemma Eq_AKE_AKE_1_O_computeKey:
+  equiv[ AKE(A).O.computeKey ~ AKE_1(A).O.computeKey :
           ( ={i} /\
-           AKE_1.evs{1}         = AKE_2.evs{2} /\
-           AKE_1.test{1}        = AKE_2.test{2} /\
-           AKE_1.cH1{1}         = AKE_2.cH1{2} /\
-           AKE_1.cH2{1}         = AKE_2.cH2{2} /\
-           AKE_1.mH1{1}         = AKE_2.mH1{2} /\
-           AKE_1.sH1{1}         = AKE_2.sH1{2} /\
-           AKE_1.mH2{1}         = AKE_2.mH2{2} /\
-           AKE_1.sH2{1}         = AKE_2.sH2{2} /\
-           AKE_1.mSk{1}         = AKE_2.mSk{2} /\
-           AKE_1.mCompleted{1}  = AKE_2.mCompleted{2} /\
-           AKE_1.bad_esk_col{1} = AKE_2.bad_esk_col{2} /\
-           AKE_1.bad_esk_norev{1} = AKE_2.bad_esk_norev{2} /\
-           eq_map_split AKE_1.mStarted{1} AKE_2.mStarted{2}
-                        AKE_2.mEsk{2} AKE_2.mEexp{2})
+           AKE.evs{1}         = AKE_1.evs{2} /\
+           AKE.test{1}        = AKE_1.test{2} /\
+           AKE.cH1{1}         = AKE_1.cH1{2} /\
+           AKE.cH2{1}         = AKE_1.cH2{2} /\
+           AKE.mH1{1}         = AKE_1.mH1{2} /\
+           AKE.sH1{1}         = AKE_1.sH1{2} /\
+           AKE.mH2{1}         = AKE_1.mH2{2} /\
+           AKE.sH2{1}         = AKE_1.sH2{2} /\
+           AKE.mSk{1}         = AKE_1.mSk{2} /\
+           AKE.mCompleted{1}  = AKE_1.mCompleted{2} /\
+           eq_map_split AKE.mStarted{1} AKE_1.mStarted{2}
+                        AKE_1.mEsk{2} AKE_1.mEexp{2})
          ==>
           ( ={res} /\
-           AKE_1.evs{1}         = AKE_2.evs{2} /\
-           AKE_1.test{1}        = AKE_2.test{2} /\
-           AKE_1.cH1{1}         = AKE_2.cH1{2} /\
-           AKE_1.cH2{1}         = AKE_2.cH2{2} /\
-           AKE_1.mH1{1}         = AKE_2.mH1{2} /\
-           AKE_1.sH1{1}         = AKE_2.sH1{2} /\
-           AKE_1.mH2{1}         = AKE_2.mH2{2} /\
-           AKE_1.sH2{1}         = AKE_2.sH2{2} /\
-           AKE_1.mSk{1}         = AKE_2.mSk{2} /\
-           AKE_1.mCompleted{1}  = AKE_2.mCompleted{2} /\
-           AKE_1.bad_esk_col{1} = AKE_2.bad_esk_col{2} /\
-           AKE_1.bad_esk_norev{1} = AKE_2.bad_esk_norev{2} /\
-           eq_map_split AKE_1.mStarted{1} AKE_2.mStarted{2}
-                        AKE_2.mEsk{2} AKE_2.mEexp{2}) ].
+           AKE.evs{1}         = AKE_1.evs{2} /\
+           AKE.test{1}        = AKE_1.test{2} /\
+           AKE.cH1{1}         = AKE_1.cH1{2} /\
+           AKE.cH2{1}         = AKE_1.cH2{2} /\
+           AKE.mH1{1}         = AKE_1.mH1{2} /\
+           AKE.sH1{1}         = AKE_1.sH1{2} /\
+           AKE.mH2{1}         = AKE_1.mH2{2} /\
+           AKE.sH2{1}         = AKE_1.sH2{2} /\
+           AKE.mSk{1}         = AKE_1.mSk{2} /\
+           AKE.mCompleted{1}  = AKE_1.mCompleted{2} /\
+           eq_map_split AKE.mStarted{1} AKE_1.mStarted{2}
+                        AKE_1.mEsk{2} AKE_1.mEexp{2}) ].
 proof strict.
   fun.
   sp.
   if ;[ by smt | | by skip; smt ].
   wp.
-  call (Eq_AKE_1_AKE_2_O_h2 A).
+  call (Eq_AKE_AKE_1_O_h2).
   wp; skip. progress.
     by generalize H; rewrite eq_map_split_def; smt.
     by smt.
 qed.
 
-lemma Eq_AKE_1_AKE_2_O_sessionRev(A <: Adv{AKE, AKE_1}):
-  equiv[ AKE_1(A).O.sessionRev ~ AKE_2(A).O.sessionRev :
+local
+lemma Eq_AKE_AKE_1_O_sessionRev:
+  equiv[ AKE(A).O.sessionRev ~ AKE_1(A).O.sessionRev :
           ( ={i} /\
-           AKE_1.evs{1}         = AKE_2.evs{2} /\
-           AKE_1.test{1}        = AKE_2.test{2} /\
-           AKE_1.cH1{1}         = AKE_2.cH1{2} /\
-           AKE_1.cH2{1}         = AKE_2.cH2{2} /\
-           AKE_1.mH1{1}         = AKE_2.mH1{2} /\
-           AKE_1.sH1{1}         = AKE_2.sH1{2} /\
-           AKE_1.mH2{1}         = AKE_2.mH2{2} /\
-           AKE_1.sH2{1}         = AKE_2.sH2{2} /\
-           AKE_1.mSk{1}         = AKE_2.mSk{2} /\
-           AKE_1.mCompleted{1}  = AKE_2.mCompleted{2} /\
-           AKE_1.bad_esk_col{1} = AKE_2.bad_esk_col{2} /\
-           AKE_1.bad_esk_norev{1} = AKE_2.bad_esk_norev{2} /\
-           eq_map_split AKE_1.mStarted{1} AKE_2.mStarted{2}
-                        AKE_2.mEsk{2} AKE_2.mEexp{2})
+           AKE.evs{1}         = AKE_1.evs{2} /\
+           AKE.test{1}        = AKE_1.test{2} /\
+           AKE.cH1{1}         = AKE_1.cH1{2} /\
+           AKE.cH2{1}         = AKE_1.cH2{2} /\
+           AKE.mH1{1}         = AKE_1.mH1{2} /\
+           AKE.sH1{1}         = AKE_1.sH1{2} /\
+           AKE.mH2{1}         = AKE_1.mH2{2} /\
+           AKE.sH2{1}         = AKE_1.sH2{2} /\
+           AKE.mSk{1}         = AKE_1.mSk{2} /\
+           AKE.mCompleted{1}  = AKE_1.mCompleted{2} /\
+           eq_map_split AKE.mStarted{1} AKE_1.mStarted{2}
+                        AKE_1.mEsk{2} AKE_1.mEexp{2})
          ==>
          ( ={res} /\
-           AKE_1.evs{1}         = AKE_2.evs{2} /\
-           AKE_1.test{1}        = AKE_2.test{2} /\
-           AKE_1.cH1{1}         = AKE_2.cH1{2} /\
-           AKE_1.cH2{1}         = AKE_2.cH2{2} /\
-           AKE_1.mH1{1}         = AKE_2.mH1{2} /\
-           AKE_1.sH1{1}         = AKE_2.sH1{2} /\
-           AKE_1.mH2{1}         = AKE_2.mH2{2} /\
-           AKE_1.sH2{1}         = AKE_2.sH2{2} /\
-           AKE_1.mSk{1}         = AKE_2.mSk{2} /\
-           AKE_1.mCompleted{1}  = AKE_2.mCompleted{2} /\
-           AKE_1.bad_esk_col{1} = AKE_2.bad_esk_col{2} /\
-           AKE_1.bad_esk_norev{1} = AKE_2.bad_esk_norev{2} /\
-           eq_map_split AKE_1.mStarted{1} AKE_2.mStarted{2}
-                        AKE_2.mEsk{2} AKE_2.mEexp{2}) ].
+           AKE.evs{1}         = AKE_1.evs{2} /\
+           AKE.test{1}        = AKE_1.test{2} /\
+           AKE.cH1{1}         = AKE_1.cH1{2} /\
+           AKE.cH2{1}         = AKE_1.cH2{2} /\
+           AKE.mH1{1}         = AKE_1.mH1{2} /\
+           AKE.sH1{1}         = AKE_1.sH1{2} /\
+           AKE.mH2{1}         = AKE_1.mH2{2} /\
+           AKE.sH2{1}         = AKE_1.sH2{2} /\
+           AKE.mSk{1}         = AKE_1.mSk{2} /\
+           AKE.mCompleted{1}  = AKE_1.mCompleted{2} /\
+           eq_map_split AKE.mStarted{1} AKE_1.mStarted{2}
+                        AKE_1.mEsk{2} AKE_1.mEexp{2}) ].
 proof strict.
   fun.
   sp.
   if; [ by smt | | by skip; smt ]. 
-  call (Eq_AKE_1_AKE_2_O_computeKey A).
+  call Eq_AKE_AKE_1_O_computeKey.
   wp; skip. smt.
 qed.
 
-lemma Eq_AKE_1_AKE_2_O_h1_a(A <: Adv{AKE, AKE_1}):
-  equiv[ AKE_1(A).O.h1_a ~ AKE_2(A).O.h1_a :
+local
+lemma Eq_AKE_AKE_1_O_h1_a:
+  equiv[ AKE(A).O.h1_a ~ AKE_1(A).O.h1_a :
          ( ={a,x} /\
-           AKE_1.evs{1}         = AKE_2.evs{2} /\
-           AKE_1.test{1}        = AKE_2.test{2} /\
-           AKE_1.cH1{1}         = AKE_2.cH1{2} /\
-           AKE_1.cH2{1}         = AKE_2.cH2{2} /\
-           AKE_1.mH1{1}         = AKE_2.mH1{2} /\
-           AKE_1.sH1{1}         = AKE_2.sH1{2} /\
-           AKE_1.mH2{1}         = AKE_2.mH2{2} /\
-           AKE_1.sH2{1}         = AKE_2.sH2{2} /\
-           AKE_1.mSk{1}         = AKE_2.mSk{2} /\
-           AKE_1.mCompleted{1}  = AKE_2.mCompleted{2} /\
-           AKE_1.bad_esk_col{1} = AKE_2.bad_esk_col{2} /\
-           AKE_1.bad_esk_norev{1} = AKE_2.bad_esk_norev{2} /\
-           eq_map_split AKE_1.mStarted{1} AKE_2.mStarted{2}
-                        AKE_2.mEsk{2} AKE_2.mEexp{2})
+           AKE.evs{1}         = AKE_1.evs{2} /\
+           AKE.test{1}        = AKE_1.test{2} /\
+           AKE.cH1{1}         = AKE_1.cH1{2} /\
+           AKE.cH2{1}         = AKE_1.cH2{2} /\
+           AKE.mH1{1}         = AKE_1.mH1{2} /\
+           AKE.sH1{1}         = AKE_1.sH1{2} /\
+           AKE.mH2{1}         = AKE_1.mH2{2} /\
+           AKE.sH2{1}         = AKE_1.sH2{2} /\
+           AKE.mSk{1}         = AKE_1.mSk{2} /\
+           AKE.mCompleted{1}  = AKE_1.mCompleted{2} /\
+           eq_map_split AKE.mStarted{1} AKE_1.mStarted{2}
+                        AKE_1.mEsk{2} AKE_1.mEexp{2})
          ==>
          ( ={res} /\
-           AKE_1.evs{1}         = AKE_2.evs{2} /\
-           AKE_1.test{1}        = AKE_2.test{2} /\
-           AKE_1.cH1{1}         = AKE_2.cH1{2} /\
-           AKE_1.cH2{1}         = AKE_2.cH2{2} /\
-           AKE_1.mH1{1}         = AKE_2.mH1{2} /\
-           AKE_1.sH1{1}         = AKE_2.sH1{2} /\
-           AKE_1.mH2{1}         = AKE_2.mH2{2} /\
-           AKE_1.sH2{1}         = AKE_2.sH2{2} /\
-           AKE_1.mSk{1}         = AKE_2.mSk{2} /\
-           AKE_1.mCompleted{1}  = AKE_2.mCompleted{2} /\
-           AKE_1.bad_esk_col{1} = AKE_2.bad_esk_col{2} /\
-           AKE_1.bad_esk_norev{1} = AKE_2.bad_esk_norev{2} /\
-           eq_map_split AKE_1.mStarted{1} AKE_2.mStarted{2}
-                        AKE_2.mEsk{2} AKE_2.mEexp{2}) ].
+           AKE.evs{1}         = AKE_1.evs{2} /\
+           AKE.test{1}        = AKE_1.test{2} /\
+           AKE.cH1{1}         = AKE_1.cH1{2} /\
+           AKE.cH2{1}         = AKE_1.cH2{2} /\
+           AKE.mH1{1}         = AKE_1.mH1{2} /\
+           AKE.sH1{1}         = AKE_1.sH1{2} /\
+           AKE.mH2{1}         = AKE_1.mH2{2} /\
+           AKE.sH2{1}         = AKE_1.sH2{2} /\
+           AKE.mSk{1}         = AKE_1.mSk{2} /\
+           AKE.mCompleted{1}  = AKE_1.mCompleted{2} /\
+           eq_map_split AKE.mStarted{1} AKE_1.mStarted{2}
+                        AKE_1.mEsk{2} AKE_1.mEexp{2}) ].
 proof strict.
   fun.
   sp.
   if; [ by smt | | by skip; smt ].
-  (* we want to use 'if' for the command setting bad *)
-  seq 1 1:
-     ( ={a,x} /\
-           AKE_1.evs{1}         = AKE_2.evs{2} /\
-           AKE_1.test{1}        = AKE_2.test{2} /\
-           AKE_1.cH1{1}         = AKE_2.cH1{2} /\
-           AKE_1.cH2{1}         = AKE_2.cH2{2} /\
-           AKE_1.mH1{1}         = AKE_2.mH1{2} /\
-           AKE_1.sH1{1}         = AKE_2.sH1{2} /\
-           AKE_1.mH2{1}         = AKE_2.mH2{2} /\
-           AKE_1.sH2{1}         = AKE_2.sH2{2} /\
-           AKE_1.mSk{1}         = AKE_2.mSk{2} /\
-           AKE_1.mCompleted{1}  = AKE_2.mCompleted{2} /\
-           AKE_1.bad_esk_col{1} = AKE_2.bad_esk_col{2} /\
-           AKE_1.bad_esk_norev{1} = AKE_2.bad_esk_norev{2} /\
-           eq_map_split AKE_1.mStarted{1} AKE_2.mStarted{2}
-                        AKE_2.mEsk{2} AKE_2.mEexp{2});
-    first by wp; skip; smt.
-  seq 2 2:
-    ( ={a,x} /\
-           AKE_1.evs{1}         = AKE_2.evs{2} /\
-           AKE_1.test{1}        = AKE_2.test{2} /\
-           AKE_1.cH1{1}         = AKE_2.cH1{2} /\
-           AKE_1.cH2{1}         = AKE_2.cH2{2} /\
-           AKE_1.mH1{1}         = AKE_2.mH1{2} /\
-           AKE_1.sH1{1}         = AKE_2.sH1{2} /\
-           AKE_1.mH2{1}         = AKE_2.mH2{2} /\
-           AKE_1.sH2{1}         = AKE_2.sH2{2} /\
-           AKE_1.mSk{1}         = AKE_2.mSk{2} /\
-           AKE_1.mCompleted{1}  = AKE_2.mCompleted{2} /\
-           AKE_1.bad_esk_col{1} = AKE_2.bad_esk_col{2} /\
-           AKE_1.bad_esk_norev{1} = AKE_2.bad_esk_norev{2} /\
-           eq_map_split AKE_1.mStarted{1} AKE_2.mStarted{2}
-                        AKE_2.mEsk{2} AKE_2.mEexp{2}).
-    if.
-      simplify.
-      intros &1 &2 H.
-      cut H1:= eq_map_split_5 AKE_1.mStarted{1} AKE_2.mStarted{2}
-                              AKE_2.mEsk{2} AKE_2.mEexp{2} AKE_2.evs{2} x{2} _. smt.
-      generalize H.
-      progress.
-      smt.
-      smt.
-    wp; skip; smt.
-    wp; skip; smt.
   wp.
-  call (Eq_AKE_1_AKE_2_O_h1 A).
-  skip; smt.
+  call Eq_AKE_AKE_1_O_h1.
+  wp; skip; smt.
 qed.
 
 (*} end: Then handle oracles that only read the modified maps*)
 
 (*{ Lastly handle oracles that write the modified maps. *)
 
-lemma Eq_AKE_1_AKE_2_O_init1(A <: Adv{AKE, AKE_1}):
-  equiv[ AKE_1(A).O.init1 ~ AKE_2(A).O.init1 :
+local
+lemma Eq_AKE_AKE_1_O_init1:
+  equiv[ AKE(A).O.init1 ~ AKE_1(A).O.init1 :
          ( ={i,A,B} /\
-           AKE_1.evs{1}         = AKE_2.evs{2} /\
-           AKE_1.test{1}        = AKE_2.test{2} /\
-           AKE_1.cH1{1}         = AKE_2.cH1{2} /\
-           AKE_1.cH2{1}         = AKE_2.cH2{2} /\
-           AKE_1.mH1{1}         = AKE_2.mH1{2} /\
-           AKE_1.sH1{1}         = AKE_2.sH1{2} /\
-           AKE_1.mH2{1}         = AKE_2.mH2{2} /\
-           AKE_1.sH2{1}         = AKE_2.sH2{2} /\
-           AKE_1.mSk{1}         = AKE_2.mSk{2} /\
-           AKE_1.mCompleted{1}  = AKE_2.mCompleted{2} /\
-           AKE_1.bad_esk_col{1} = AKE_2.bad_esk_col{2} /\
-           AKE_1.bad_esk_norev{1} = AKE_2.bad_esk_norev{2} /\
-           eq_map_split AKE_1.mStarted{1} AKE_2.mStarted{2}
-                        AKE_2.mEsk{2} AKE_2.mEexp{2})
+           AKE.evs{1}         = AKE_1.evs{2} /\
+           AKE.test{1}        = AKE_1.test{2} /\
+           AKE.cH1{1}         = AKE_1.cH1{2} /\
+           AKE.cH2{1}         = AKE_1.cH2{2} /\
+           AKE.mH1{1}         = AKE_1.mH1{2} /\
+           AKE.sH1{1}         = AKE_1.sH1{2} /\
+           AKE.mH2{1}         = AKE_1.mH2{2} /\
+           AKE.sH2{1}         = AKE_1.sH2{2} /\
+           AKE.mSk{1}         = AKE_1.mSk{2} /\
+           AKE.mCompleted{1}  = AKE_1.mCompleted{2} /\
+           eq_map_split AKE.mStarted{1} AKE_1.mStarted{2}
+                        AKE_1.mEsk{2} AKE_1.mEexp{2})
          ==>
          ( ={res} /\
-           AKE_1.evs{1}         = AKE_2.evs{2} /\
-           AKE_1.test{1}        = AKE_2.test{2} /\
-           AKE_1.cH1{1}         = AKE_2.cH1{2} /\
-           AKE_1.cH2{1}         = AKE_2.cH2{2} /\
-           AKE_1.mH1{1}         = AKE_2.mH1{2} /\
-           AKE_1.sH1{1}         = AKE_2.sH1{2} /\
-           AKE_1.mH2{1}         = AKE_2.mH2{2} /\
-           AKE_1.sH2{1}         = AKE_2.sH2{2} /\
-           AKE_1.mSk{1}         = AKE_2.mSk{2} /\
-           AKE_1.mCompleted{1}  = AKE_2.mCompleted{2} /\
-           AKE_1.bad_esk_col{1} = AKE_2.bad_esk_col{2} /\
-           AKE_1.bad_esk_norev{1} = AKE_2.bad_esk_norev{2} /\
-           eq_map_split AKE_1.mStarted{1} AKE_2.mStarted{2}
-                        AKE_2.mEsk{2} AKE_2.mEexp{2}) ].
+           AKE.evs{1}         = AKE_1.evs{2} /\
+           AKE.test{1}        = AKE_1.test{2} /\
+           AKE.cH1{1}         = AKE_1.cH1{2} /\
+           AKE.cH2{1}         = AKE_1.cH2{2} /\
+           AKE.mH1{1}         = AKE_1.mH1{2} /\
+           AKE.sH1{1}         = AKE_1.sH1{2} /\
+           AKE.mH2{1}         = AKE_1.mH2{2} /\
+           AKE.sH2{1}         = AKE_1.sH2{2} /\
+           AKE.mSk{1}         = AKE_1.mSk{2} /\
+           AKE.mCompleted{1}  = AKE_1.mCompleted{2} /\
+           eq_map_split AKE.mStarted{1} AKE_1.mStarted{2}
+                        AKE_1.mEsk{2} AKE_1.mEexp{2}) ].
 proof strict.
   fun.
   sp.
   if; [ by smt | | skip; by smt ].
-  sp.
-  swap {2} 2 1.
   wp.
-  call (Eq_AKE_1_AKE_2_O_h1 A).
-  seq 1 1:
-    ( ={i,A,B,r,x} /\
-     AKE_1.evs{1}         = AKE_2.evs{2} /\
-     AKE_1.test{1}        = AKE_2.test{2} /\
-     AKE_1.cH1{1}         = AKE_2.cH1{2} /\
-     AKE_1.cH2{1}         = AKE_2.cH2{2} /\
-     AKE_1.mH1{1}         = AKE_2.mH1{2} /\
-     AKE_1.sH1{1}         = AKE_2.sH1{2} /\
-     AKE_1.mH2{1}         = AKE_2.mH2{2} /\
-     AKE_1.sH2{1}         = AKE_2.sH2{2} /\
-     AKE_1.mSk{1}         = AKE_2.mSk{2} /\
-     AKE_1.mCompleted{1}  = AKE_2.mCompleted{2} /\
-     AKE_1.bad_esk_col{1} = AKE_2.bad_esk_col{2} /\
-     AKE_1.bad_esk_norev{1} = AKE_2.bad_esk_norev{2} /\
-     eq_map_split AKE_1.mStarted{1} AKE_2.mStarted{2}
-                  AKE_2.mEsk{2} AKE_2.mEexp{2}).
-  rnd; skip; smt.
-  seq 1 1:
-    ( ={i,A,B,r,x} /\
-     AKE_1.evs{1}         = AKE_2.evs{2} /\
-     AKE_1.test{1}        = AKE_2.test{2} /\
-     AKE_1.cH1{1}         = AKE_2.cH1{2} /\
-     AKE_1.cH2{1}         = AKE_2.cH2{2} /\
-     AKE_1.mH1{1}         = AKE_2.mH1{2} /\
-     AKE_1.sH1{1}         = AKE_2.sH1{2} /\
-     AKE_1.mH2{1}         = AKE_2.mH2{2} /\
-     AKE_1.sH2{1}         = AKE_2.sH2{2} /\
-     AKE_1.mSk{1}         = AKE_2.mSk{2} /\
-     AKE_1.mCompleted{1}  = AKE_2.mCompleted{2} /\
-     AKE_1.bad_esk_col{1} = AKE_2.bad_esk_col{2} /\
-     AKE_1.bad_esk_norev{1} = AKE_2.bad_esk_norev{2} /\
-     eq_map_split AKE_1.mStarted{1} AKE_2.mStarted{2}
-                  AKE_2.mEsk{2} AKE_2.mEexp{2}).
-  if; [ by smt | | by skip; smt ].
-    by wp; skip; smt.
-  wp. skip. progress. smt. smt.
+  call Eq_AKE_AKE_1_O_h1.
+  wp.
+  rnd.
+  skip; progress. smt. smt. smt. 
   generalize H.
-  rewrite !eq_map_split_def.
-  progress. smt. smt. smt. smt. smt. 
+  rewrite !eq_map_split_def. progress. smt. smt. smt. smt. smt.
   case (i{2} = i0).
     intros eq. rewrite !eq !get_setE; smt.
-  intros neq. rewrite !get_setNE. smt. smt.
-    generalize H3.
-    rewrite (in_dom_setNE i0 AKE_1.mStarted{1}). smt. smt.
+  intros neq. rewrite !get_setNE. smt. smt. 
+    generalize H9.
+    rewrite (in_dom_setNE i0 AKE.mStarted{1}). smt. smt.
   smt.
   smt.
 qed.
 
-lemma Eq_AKE_1_AKE_2_O_resp(A <: Adv{AKE, AKE_1}):
-  equiv[ AKE_1(A).O.resp ~ AKE_2(A).O.resp :
+local
+lemma Eq_AKE_AKE_1_O_resp:
+  equiv[ AKE(A).O.resp ~ AKE_1(A).O.resp :
          ( ={i, B, A, X} /\
-           AKE_1.evs{1}         = AKE_2.evs{2} /\
-           AKE_1.test{1}        = AKE_2.test{2} /\
-           AKE_1.cH1{1}         = AKE_2.cH1{2} /\
-           AKE_1.cH2{1}         = AKE_2.cH2{2} /\
-           AKE_1.mH1{1}         = AKE_2.mH1{2} /\
-           AKE_1.sH1{1}         = AKE_2.sH1{2} /\
-           AKE_1.mH2{1}         = AKE_2.mH2{2} /\
-           AKE_1.sH2{1}         = AKE_2.sH2{2} /\
-           AKE_1.mSk{1}         = AKE_2.mSk{2} /\
-           AKE_1.mCompleted{1}  = AKE_2.mCompleted{2} /\
-           AKE_1.bad_esk_col{1} = AKE_2.bad_esk_col{2} /\
-           AKE_1.bad_esk_norev{1} = AKE_2.bad_esk_norev{2} /\
-           eq_map_split AKE_1.mStarted{1} AKE_2.mStarted{2}
-                        AKE_2.mEsk{2} AKE_2.mEexp{2})
+           AKE.evs{1}         = AKE_1.evs{2} /\
+           AKE.test{1}        = AKE_1.test{2} /\
+           AKE.cH1{1}         = AKE_1.cH1{2} /\
+           AKE.cH2{1}         = AKE_1.cH2{2} /\
+           AKE.mH1{1}         = AKE_1.mH1{2} /\
+           AKE.sH1{1}         = AKE_1.sH1{2} /\
+           AKE.mH2{1}         = AKE_1.mH2{2} /\
+           AKE.sH2{1}         = AKE_1.sH2{2} /\
+           AKE.mSk{1}         = AKE_1.mSk{2} /\
+           AKE.mCompleted{1}  = AKE_1.mCompleted{2} /\
+           eq_map_split AKE.mStarted{1} AKE_1.mStarted{2}
+                        AKE_1.mEsk{2} AKE_1.mEexp{2})
          ==>
          ( ={res} /\
-           AKE_1.evs{1}         = AKE_2.evs{2} /\
-           AKE_1.test{1}        = AKE_2.test{2} /\
-           AKE_1.cH1{1}         = AKE_2.cH1{2} /\
-           AKE_1.cH2{1}         = AKE_2.cH2{2} /\
-           AKE_1.mH1{1}         = AKE_2.mH1{2} /\
-           AKE_1.sH1{1}         = AKE_2.sH1{2} /\
-           AKE_1.mH2{1}         = AKE_2.mH2{2} /\
-           AKE_1.sH2{1}         = AKE_2.sH2{2} /\
-           AKE_1.mSk{1}         = AKE_2.mSk{2} /\
-           AKE_1.mCompleted{1}  = AKE_2.mCompleted{2} /\
-           AKE_1.bad_esk_col{1} = AKE_2.bad_esk_col{2} /\
-           AKE_1.bad_esk_norev{1} = AKE_2.bad_esk_norev{2} /\
-           eq_map_split AKE_1.mStarted{1} AKE_2.mStarted{2}
-                        AKE_2.mEsk{2} AKE_2.mEexp{2}) ].
+           AKE.evs{1}         = AKE_1.evs{2} /\
+           AKE.test{1}        = AKE_1.test{2} /\
+           AKE.cH1{1}         = AKE_1.cH1{2} /\
+           AKE.cH2{1}         = AKE_1.cH2{2} /\
+           AKE.mH1{1}         = AKE_1.mH1{2} /\
+           AKE.sH1{1}         = AKE_1.sH1{2} /\
+           AKE.mH2{1}         = AKE_1.mH2{2} /\
+           AKE.sH2{1}         = AKE_1.sH2{2} /\
+           AKE.mSk{1}         = AKE_1.mSk{2} /\
+           AKE.mCompleted{1}  = AKE_1.mCompleted{2} /\
+           eq_map_split AKE.mStarted{1} AKE_1.mStarted{2}
+                        AKE_1.mEsk{2} AKE_1.mEexp{2}) ].
 proof strict.
   fun.
   sp.
   if; [ by smt | | skip; by smt ].
   wp.
-  call (Eq_AKE_1_AKE_2_O_h1 A).
-  swap {2} 2 1.
-  sp.
-  seq 1 1 :
-    ( ={i,A,B,r,y,X} /\
-     AKE_1.evs{1}         = AKE_2.evs{2} /\
-     AKE_1.test{1}        = AKE_2.test{2} /\
-     AKE_1.cH1{1}         = AKE_2.cH1{2} /\
-     AKE_1.cH2{1}         = AKE_2.cH2{2} /\
-     AKE_1.mH1{1}         = AKE_2.mH1{2} /\
-     AKE_1.sH1{1}         = AKE_2.sH1{2} /\
-     AKE_1.mH2{1}         = AKE_2.mH2{2} /\
-     AKE_1.sH2{1}         = AKE_2.sH2{2} /\
-     AKE_1.mSk{1}         = AKE_2.mSk{2} /\
-     AKE_1.mCompleted{1}  = AKE_2.mCompleted{2} /\
-     AKE_1.bad_esk_col{1} = AKE_2.bad_esk_col{2} /\
-     AKE_1.bad_esk_norev{1} = AKE_2.bad_esk_norev{2} /\
-     eq_map_split AKE_1.mStarted{1} AKE_2.mStarted{2}
-                  AKE_2.mEsk{2} AKE_2.mEexp{2}).
-  rnd. skip. smt.
-  seq 1 1 :
-    ( ={i,A,B,r,y,X} /\
-     AKE_1.evs{1}         = AKE_2.evs{2} /\
-     AKE_1.test{1}        = AKE_2.test{2} /\
-     AKE_1.cH1{1}         = AKE_2.cH1{2} /\
-     AKE_1.cH2{1}         = AKE_2.cH2{2} /\
-     AKE_1.mH1{1}         = AKE_2.mH1{2} /\
-     AKE_1.sH1{1}         = AKE_2.sH1{2} /\
-     AKE_1.mH2{1}         = AKE_2.mH2{2} /\
-     AKE_1.sH2{1}         = AKE_2.sH2{2} /\
-     AKE_1.mSk{1}         = AKE_2.mSk{2} /\
-     AKE_1.mCompleted{1}  = AKE_2.mCompleted{2} /\
-     AKE_1.bad_esk_col{1} = AKE_2.bad_esk_col{2} /\
-     AKE_1.bad_esk_norev{1} = AKE_2.bad_esk_norev{2} /\
-     eq_map_split AKE_1.mStarted{1} AKE_2.mStarted{2}
-                  AKE_2.mEsk{2} AKE_2.mEexp{2}).
-  if. smt. wp; skip; smt. skip; smt.
-  wp; skip.
-  simplify.
-  intros &1 &2 H.
-  generalize H.
-  progress.
-    smt.
-    smt.
+  call Eq_AKE_AKE_1_O_h1.
+  wp.
+  rnd; skip; progress. smt. smt. smt.
   generalize H. rewrite !eq_map_split_def.
   progress.
     smt. smt. smt. smt. smt.
   case (i{2} = i0).
     intros eq. rewrite !eq !get_setE; smt.
   intros neq. rewrite !get_setNE. smt. smt.
-    generalize H3.
-    rewrite (in_dom_setNE i0 AKE_1.mStarted{1}). smt. smt.
+    generalize H10.
+    rewrite (in_dom_setNE i0 AKE.mStarted{1}). smt. smt.
   smt.
   smt.
 qed.
 
 (*} end: Lastly handle oracles that write the modified maps. *)
 
-lemma Eq_AKE_1_AKE_2(A <: Adv{AKE_1, AKE_2}):
-  equiv[ AKE_1(A).main ~ AKE_2(A).main : true ==>
-            (res /\ test_fresh AKE_1.test AKE_1.evs /\
-             !AKE_1.bad_esk_col /\ !AKE_1.bad_esk_norev){1}
-         => (res /\ test_fresh AKE_2.test AKE_2.evs /\
-             !AKE_2.bad_esk_col /\ !AKE_2.bad_esk_norev){2} ].
+local
+lemma Eq_AKE_AKE_1:
+  equiv[ AKE(A).main ~ AKE_1(A).main : true ==>
+            (res /\ test_fresh AKE.test AKE.evs){1}
+         => (res /\ test_fresh AKE_1.test AKE_1.evs){2} ].
 proof strict.
   fun.
-  inline AKE_1(A).init AKE_2(A).init.
-  seq 22 24:
+  inline AKE(A).init AKE_1(A).init.
+  seq 20 22:
     ( ={b,pks,t_idx,key,keyo,b',i,ska,pka} /\
-      AKE_1.evs{1}         = AKE_2.evs{2} /\
-      AKE_1.test{1}        = AKE_2.test{2} /\
-      AKE_1.cH1{1}         = AKE_2.cH1{2} /\
-      AKE_1.cH2{1}         = AKE_2.cH2{2} /\
-      AKE_1.mH1{1}         = AKE_2.mH1{2} /\
-      AKE_1.sH1{1}         = AKE_2.sH1{2} /\
-      AKE_1.mH2{1}         = AKE_2.mH2{2} /\
-      AKE_1.sH2{1}         = AKE_2.sH2{2} /\
-      AKE_1.mSk{1}         = AKE_2.mSk{2} /\
-      AKE_1.mCompleted{1}  = AKE_2.mCompleted{2} /\
-      AKE_1.bad_esk_col{1} = AKE_2.bad_esk_col{2} /\
-      AKE_1.bad_esk_norev{1} = AKE_2.bad_esk_norev{2} /\
-      eq_map_split AKE_1.mStarted{1} AKE_2.mStarted{2}
-                   AKE_2.mEsk{2} AKE_2.mEexp{2}).
+      AKE.evs{1}         = AKE_1.evs{2} /\
+      AKE.test{1}        = AKE_1.test{2} /\
+      AKE.cH1{1}         = AKE_1.cH1{2} /\
+      AKE.cH2{1}         = AKE_1.cH2{2} /\
+      AKE.mH1{1}         = AKE_1.mH1{2} /\
+      AKE.sH1{1}         = AKE_1.sH1{2} /\
+      AKE.mH2{1}         = AKE_1.mH2{2} /\
+      AKE.sH2{1}         = AKE_1.sH2{2} /\
+      AKE.mSk{1}         = AKE_1.mSk{2} /\
+      AKE.mCompleted{1}  = AKE_1.mCompleted{2} /\
+      eq_map_split AKE.mStarted{1} AKE_1.mStarted{2}
+                   AKE_1.mEsk{2} AKE_1.mEexp{2}).
   by wp; skip; rewrite eq_map_split_def; smt.
   seq 1 1:
     ( ={b,pks,t_idx,key,keyo,b',i,ska,pka} /\
-      AKE_1.evs{1}         = AKE_2.evs{2} /\
-      AKE_1.test{1}        = AKE_2.test{2} /\
-      AKE_1.cH1{1}         = AKE_2.cH1{2} /\
-      AKE_1.cH2{1}         = AKE_2.cH2{2} /\
-      AKE_1.mH1{1}         = AKE_2.mH1{2} /\
-      AKE_1.sH1{1}         = AKE_2.sH1{2} /\
-      AKE_1.mH2{1}         = AKE_2.mH2{2} /\
-      AKE_1.sH2{1}         = AKE_2.sH2{2} /\
-      AKE_1.mSk{1}         = AKE_2.mSk{2} /\
-      AKE_1.mCompleted{1}  = AKE_2.mCompleted{2} /\
-      AKE_1.bad_esk_col{1} = AKE_2.bad_esk_col{2} /\
-      AKE_1.bad_esk_norev{1} = AKE_2.bad_esk_norev{2} /\
-      eq_map_split AKE_1.mStarted{1} AKE_2.mStarted{2}
-                   AKE_2.mEsk{2} AKE_2.mEexp{2}).
+      AKE.evs{1}         = AKE_1.evs{2} /\
+      AKE.test{1}        = AKE_1.test{2} /\
+      AKE.cH1{1}         = AKE_1.cH1{2} /\
+      AKE.cH2{1}         = AKE_1.cH2{2} /\
+      AKE.mH1{1}         = AKE_1.mH1{2} /\
+      AKE.sH1{1}         = AKE_1.sH1{2} /\
+      AKE.mH2{1}         = AKE_1.mH2{2} /\
+      AKE.sH2{1}         = AKE_1.sH2{2} /\
+      AKE.mSk{1}         = AKE_1.mSk{2} /\
+      AKE.mCompleted{1}  = AKE_1.mCompleted{2} /\
+      eq_map_split AKE.mStarted{1} AKE_1.mStarted{2}
+                   AKE_1.mEsk{2} AKE_1.mEexp{2}).
   while 
     ( ={b,pks,t_idx,key,keyo,b',i,ska,pka} /\
-      AKE_1.evs{1}         = AKE_2.evs{2} /\
-      AKE_1.test{1}        = AKE_2.test{2} /\
-      AKE_1.cH1{1}         = AKE_2.cH1{2} /\
-      AKE_1.cH2{1}         = AKE_2.cH2{2} /\
-      AKE_1.mH1{1}         = AKE_2.mH1{2} /\
-      AKE_1.sH1{1}         = AKE_2.sH1{2} /\
-      AKE_1.mH2{1}         = AKE_2.mH2{2} /\
-      AKE_1.sH2{1}         = AKE_2.sH2{2} /\
-      AKE_1.mSk{1}         = AKE_2.mSk{2} /\
-      AKE_1.mCompleted{1}  = AKE_2.mCompleted{2} /\
-      AKE_1.bad_esk_col{1} = AKE_2.bad_esk_col{2} /\
-      AKE_1.bad_esk_norev{1} = AKE_2.bad_esk_norev{2} /\
-      eq_map_split AKE_1.mStarted{1} AKE_2.mStarted{2}
-                   AKE_2.mEsk{2} AKE_2.mEexp{2}).
-  by wp; rnd; skip; smt.
+      AKE.evs{1}         = AKE_1.evs{2} /\
+      AKE.test{1}        = AKE_1.test{2} /\
+      AKE.cH1{1}         = AKE_1.cH1{2} /\
+      AKE.cH2{1}         = AKE_1.cH2{2} /\
+      AKE.mH1{1}         = AKE_1.mH1{2} /\
+      AKE.sH1{1}         = AKE_1.sH1{2} /\
+      AKE.mH2{1}         = AKE_1.mH2{2} /\
+      AKE.sH2{1}         = AKE_1.sH2{2} /\
+      AKE.mSk{1}         = AKE_1.mSk{2} /\
+      AKE.mCompleted{1}  = AKE_1.mCompleted{2} /\
+      eq_map_split AKE.mStarted{1} AKE_1.mStarted{2}
+                   AKE_1.mEsk{2} AKE_1.mEexp{2}).  
+  by wp; rnd; wp; skip; smt.
   by skip; smt.
   seq 1 1:
     ( ={b,pks,t_idx,key,keyo,b',i,ska,pka} /\
-      AKE_1.evs{1}         = AKE_2.evs{2} /\
-      AKE_1.test{1}        = AKE_2.test{2} /\
-      AKE_1.cH1{1}         = AKE_2.cH1{2} /\
-      AKE_1.cH2{1}         = AKE_2.cH2{2} /\
-      AKE_1.mH1{1}         = AKE_2.mH1{2} /\
-      AKE_1.sH1{1}         = AKE_2.sH1{2} /\
-      AKE_1.mH2{1}         = AKE_2.mH2{2} /\
-      AKE_1.sH2{1}         = AKE_2.sH2{2} /\
-      AKE_1.mSk{1}         = AKE_2.mSk{2} /\
-      AKE_1.mCompleted{1}  = AKE_2.mCompleted{2} /\
-      AKE_1.bad_esk_col{1} = AKE_2.bad_esk_col{2} /\
-      AKE_1.bad_esk_norev{1} = AKE_2.bad_esk_norev{2} /\
-      eq_map_split AKE_1.mStarted{1} AKE_2.mStarted{2}
-                   AKE_2.mEsk{2} AKE_2.mEexp{2} /\
+      AKE.evs{1}         = AKE_1.evs{2} /\
+      AKE.test{1}        = AKE_1.test{2} /\
+      AKE.cH1{1}         = AKE_1.cH1{2} /\
+      AKE.cH2{1}         = AKE_1.cH2{2} /\
+      AKE.mH1{1}         = AKE_1.mH1{2} /\
+      AKE.sH1{1}         = AKE_1.sH1{2} /\
+      AKE.mH2{1}         = AKE_1.mH2{2} /\
+      AKE.sH2{1}         = AKE_1.sH2{2} /\
+      AKE.mSk{1}         = AKE_1.mSk{2} /\
+      AKE.mCompleted{1}  = AKE_1.mCompleted{2} /\
+      eq_map_split AKE.mStarted{1} AKE_1.mStarted{2}
+                   AKE_1.mEsk{2} AKE_1.mEexp{2} /\
       ={glob A}).
   call 
      (_: 
-      AKE_1.evs{1}         = AKE_2.evs{2} /\
-      AKE_1.test{1}        = AKE_2.test{2} /\
-      AKE_1.cH1{1}         = AKE_2.cH1{2} /\
-      AKE_1.cH2{1}         = AKE_2.cH2{2} /\
-      AKE_1.mH1{1}         = AKE_2.mH1{2} /\
-      AKE_1.sH1{1}         = AKE_2.sH1{2} /\
-      AKE_1.mH2{1}         = AKE_2.mH2{2} /\
-      AKE_1.sH2{1}         = AKE_2.sH2{2} /\
-      AKE_1.mSk{1}         = AKE_2.mSk{2} /\
-      AKE_1.mCompleted{1}  = AKE_2.mCompleted{2} /\
-      AKE_1.bad_esk_col{1} = AKE_2.bad_esk_col{2} /\
-      AKE_1.bad_esk_norev{1} = AKE_2.bad_esk_norev{2} /\
-      eq_map_split AKE_1.mStarted{1} AKE_2.mStarted{2}
-                   AKE_2.mEsk{2} AKE_2.mEexp{2}).
-    apply (Eq_AKE_1_AKE_2_O_h1_a A).
-    apply (Eq_AKE_1_AKE_2_O_h2_a A).
-    apply (Eq_AKE_1_AKE_2_O_init1 A).
-    apply (Eq_AKE_1_AKE_2_O_init2 A).
-    apply (Eq_AKE_1_AKE_2_O_resp A).
-    apply (Eq_AKE_1_AKE_2_O_staticRev A).
-    apply (Eq_AKE_1_AKE_2_O_ephemeralRev A).
-    apply (Eq_AKE_1_AKE_2_O_sessionRev A).
+      AKE.evs{1}         = AKE_1.evs{2} /\
+      AKE.test{1}        = AKE_1.test{2} /\
+      AKE.cH1{1}         = AKE_1.cH1{2} /\
+      AKE.cH2{1}         = AKE_1.cH2{2} /\
+      AKE.mH1{1}         = AKE_1.mH1{2} /\
+      AKE.sH1{1}         = AKE_1.sH1{2} /\
+      AKE.mH2{1}         = AKE_1.mH2{2} /\
+      AKE.sH2{1}         = AKE_1.sH2{2} /\
+      AKE.mSk{1}         = AKE_1.mSk{2} /\
+      AKE.mCompleted{1}  = AKE_1.mCompleted{2} /\
+      eq_map_split AKE.mStarted{1} AKE_1.mStarted{2}
+                   AKE_1.mEsk{2} AKE_1.mEexp{2}).
+    apply Eq_AKE_AKE_1_O_h1_a.
+    apply Eq_AKE_AKE_1_O_h2_a.
+    apply Eq_AKE_AKE_1_O_init1.
+    apply Eq_AKE_AKE_1_O_init2.
+    apply Eq_AKE_AKE_1_O_resp.
+    apply Eq_AKE_AKE_1_O_staticRev.
+    apply Eq_AKE_AKE_1_O_ephemeralRev.
+    apply Eq_AKE_AKE_1_O_sessionRev.
     by skip; smt.
     seq 1 1:
     ( ={b,pks,t_idx,key,keyo,b',i,ska,pka} /\
-      AKE_1.evs{1}         = AKE_2.evs{2} /\
-      AKE_1.test{1}        = AKE_2.test{2} /\
-      AKE_1.cH1{1}         = AKE_2.cH1{2} /\
-      AKE_1.cH2{1}         = AKE_2.cH2{2} /\
-      AKE_1.mH1{1}         = AKE_2.mH1{2} /\
-      AKE_1.sH1{1}         = AKE_2.sH1{2} /\
-      AKE_1.mH2{1}         = AKE_2.mH2{2} /\
-      AKE_1.sH2{1}         = AKE_2.sH2{2} /\
-      AKE_1.mSk{1}         = AKE_2.mSk{2} /\
-      AKE_1.mCompleted{1}  = AKE_2.mCompleted{2} /\
-      AKE_1.bad_esk_col{1} = AKE_2.bad_esk_col{2} /\
-      AKE_1.bad_esk_norev{1} = AKE_2.bad_esk_norev{2} /\
-      eq_map_split AKE_1.mStarted{1} AKE_2.mStarted{2}
-                   AKE_2.mEsk{2} AKE_2.mEexp{2} /\
+      AKE.evs{1}         = AKE_1.evs{2} /\
+      AKE.test{1}        = AKE_1.test{2} /\
+      AKE.cH1{1}         = AKE_1.cH1{2} /\
+      AKE.cH2{1}         = AKE_1.cH2{2} /\
+      AKE.mH1{1}         = AKE_1.mH1{2} /\
+      AKE.sH1{1}         = AKE_1.sH1{2} /\
+      AKE.mH2{1}         = AKE_1.mH2{2} /\
+      AKE.sH2{1}         = AKE_1.sH2{2} /\
+      AKE.mSk{1}         = AKE_1.mSk{2} /\
+      AKE.mCompleted{1}  = AKE_1.mCompleted{2} /\
+      eq_map_split AKE.mStarted{1} AKE_1.mStarted{2}
+                   AKE_1.mEsk{2} AKE_1.mEexp{2} /\
       ={glob A}).
     by rnd; skip; smt.
     if; [ by smt | | by skip; smt ].
     call 
      (_: 
-      AKE_1.evs{1}         = AKE_2.evs{2} /\
-      AKE_1.test{1}        = AKE_2.test{2} /\
-      AKE_1.cH1{1}         = AKE_2.cH1{2} /\
-      AKE_1.cH2{1}         = AKE_2.cH2{2} /\
-      AKE_1.mH1{1}         = AKE_2.mH1{2} /\
-      AKE_1.sH1{1}         = AKE_2.sH1{2} /\
-      AKE_1.mH2{1}         = AKE_2.mH2{2} /\
-      AKE_1.sH2{1}         = AKE_2.sH2{2} /\
-      AKE_1.mSk{1}         = AKE_2.mSk{2} /\
-      AKE_1.mCompleted{1}  = AKE_2.mCompleted{2} /\
-      AKE_1.bad_esk_col{1} = AKE_2.bad_esk_col{2} /\
-      AKE_1.bad_esk_norev{1} = AKE_2.bad_esk_norev{2} /\
-      eq_map_split AKE_1.mStarted{1} AKE_2.mStarted{2}
-                   AKE_2.mEsk{2} AKE_2.mEexp{2}).
-    apply (Eq_AKE_1_AKE_2_O_h1_a A).
-    apply (Eq_AKE_1_AKE_2_O_h2_a A).
-    apply (Eq_AKE_1_AKE_2_O_init1 A).
-    apply (Eq_AKE_1_AKE_2_O_init2 A).
-    apply (Eq_AKE_1_AKE_2_O_resp A).
-    apply (Eq_AKE_1_AKE_2_O_staticRev A).
-    apply (Eq_AKE_1_AKE_2_O_ephemeralRev A).
-    apply (Eq_AKE_1_AKE_2_O_sessionRev A).
+      AKE.evs{1}         = AKE_1.evs{2} /\
+      AKE.test{1}        = AKE_1.test{2} /\
+      AKE.cH1{1}         = AKE_1.cH1{2} /\
+      AKE.cH2{1}         = AKE_1.cH2{2} /\
+      AKE.mH1{1}         = AKE_1.mH1{2} /\
+      AKE.sH1{1}         = AKE_1.sH1{2} /\
+      AKE.mH2{1}         = AKE_1.mH2{2} /\
+      AKE.sH2{1}         = AKE_1.sH2{2} /\
+      AKE.mSk{1}         = AKE_1.mSk{2} /\
+      AKE.mCompleted{1}  = AKE_1.mCompleted{2} /\
+      eq_map_split AKE.mStarted{1} AKE_1.mStarted{2}
+                   AKE_1.mEsk{2} AKE_1.mEexp{2}).
+    apply Eq_AKE_AKE_1_O_h1_a.
+    apply Eq_AKE_AKE_1_O_h2_a.
+    apply Eq_AKE_AKE_1_O_init1.
+    apply Eq_AKE_AKE_1_O_init2.
+    apply Eq_AKE_AKE_1_O_resp.
+    apply Eq_AKE_AKE_1_O_staticRev.
+    apply Eq_AKE_AKE_1_O_ephemeralRev.
+    apply Eq_AKE_AKE_1_O_sessionRev.
     sp.
     if; first by smt.
-    call (Eq_AKE_1_AKE_2_O_computeKey A).
+    call Eq_AKE_AKE_1_O_computeKey.
     by skip; progress; smt.
     by wp; rnd; skip; progress; smt.
 qed.
 
 (* Move sampling of ephemeral exponents to loop in main.
-   Can be justified by making domain finite (subtype of int)
-   and using lazy/eager RO transformation.
+   Can be justified with the lazy/eager RO transformation.
 *)
+local
+module AKE_2(FA : Adv) = {
+  
+  var evs  : Event list               (* events for queries performed by adversary *)
+  var test : Sid option               (* session id of test session *)
+
+  var cH1, cH2 : int                  (* counters for queries *)
+
+  var mH1 : ((Sk * Esk), Eexp) map    (* map for h1 *)
+  var sH1 : (Sk * Esk) set            (* adversary queries for h1 *)
+
+  var mH2 : (Sstring, Key) map        (* map for h2 *)
+  var sH2 : Sstring set               (* adversary queries for h2 *)
+
+  var mSk        : (Agent, Sk) map    (* map for static secret keys *)
+  var mEsk       : (Sidx, Esk) map    (* map for ephemeral secret keys *)
+  var mEexp      : (Sidx, Eexp) map   (* map for ephemeral exponents of sessions *)
+  var mStarted   : (Sidx, Sdata2) map (* map of started sessions *)
+  var mCompleted : (Sidx, Epk)   map  (* additional data for completed sessions *)
+
+  fun init() : unit = {
+    evs = [];
+    test = None;
+    cH1 = 0;
+    cH2 = 0;
+    mH1 = Map.empty;
+    sH1 = FSet.empty;
+    mH2 = Map.empty;
+    sH2 = FSet.empty;
+    mSk = Map.empty;
+    mEsk = Map.empty;
+    mEexp = Map.empty;
+    mStarted = Map.empty;
+    mCompleted = Map.empty;
+  }
+
+  module O : AKE_Oracles = {
+
+    fun h1(a : Sk, x : Esk) : Eexp = {
+      var e : Eexp;
+      e = $sample_Eexp;
+      if (!in_dom (a,x) mH1) {
+        mH1.[(a,x)] = e;
+      } 
+      return proj mH1.[(a,x)];
+    }
+
+    fun h1_a(a : Sk, x : Esk) : Eexp option = {
+      var r : Eexp option = None;
+      var xe : Eexp;
+      if (cH1 < qH1) {
+        cH1 = cH1 + 1;
+        sH1 = add (a,x) sH1;
+        xe = h1(a,x);
+        r = Some(xe);
+      }
+      return r;
+    }
+
+    fun h2(sstring : Sstring) : Key = {
+      var ke : Key;
+      ke = $sample_Key;
+      if (!in_dom sstring mH2) {
+        mH2.[sstring] = ke;
+      }
+      return proj mH2.[sstring];
+    }
+ 
+    fun h2_a(sstring : Sstring) : Key option = {
+      var r : Key option = None;
+      var ks : Key;
+      if (cH2 < qH2) {
+        cH2 = cH2 + 1;
+        sH2 = add sstring sH2;
+        ks = h2(sstring);
+        r = Some(ks);
+      }
+      return r;
+    }
+
+    fun init1(i : Sidx, A : Agent, B : Agent) : Epk option = {
+      var pX : Epk;
+      var x : Esk;
+      var r : Epk option = None; 
+      if (in_dom A mSk && in_dom B mSk && !in_dom i mStarted) {
+        x = proj mEsk.[i];
+        mEexp.[i] = h1(proj (mSk.[A]),x);
+        pX = gen_epk(proj mEexp.[i]);
+        mStarted.[i] = (A,B,init);
+        r = Some(pX);
+        evs = Start(compute_psid mStarted mEexp i)::evs;
+      }
+      return r;
+    }
+
+    fun resp(i : Sidx, B : Agent, A : Agent, X : Epk) : Epk option = {
+      var y : Esk;
+      var pY : Epk;
+      var r : Epk option = None; 
+      if (in_dom A mSk && in_dom B mSk && !in_dom i mStarted && !in_dom i mCompleted) {
+        y = proj mEsk.[i];
+        mEexp.[i] = h1(proj (mSk.[B]),y);
+        pY = gen_epk(proj mEexp.[i]);
+        mStarted.[i] = (B,A,resp);
+        mCompleted.[i] = X;
+        r = Some(pY);
+        evs = Accept(compute_sid mStarted mEexp mCompleted i)::evs;
+      }
+      return r;
+    }
+
+    fun init2(i : Sidx, Y : Epk) : unit = {
+      if (!in_dom i mCompleted && in_dom i mStarted && in_dom i mEexp) {
+        mCompleted.[i] = Y;
+        evs = Accept(compute_sid mStarted mEexp mCompleted i)::evs;
+      }
+    }
+
+    fun staticRev(A : Agent) : Sk option = {
+      var r : Sk option = None;
+      if (in_dom A mSk) {
+        r = mSk.[A];
+        evs = StaticRev(A)::evs;
+      }
+      return r;
+    }
+
+    fun ephemeralRev(i : Sidx) : Esk option = {
+      var r : Esk option = None;
+      if (in_dom i mStarted && in_dom i mEexp) {
+        r = mEsk.[i];
+        evs = EphemeralRev(compute_psid mStarted mEexp i)::evs;
+      }
+      return r;
+    }
+
+    fun computeKey(i : Sidx) : Key option = {
+      var r : Key option = None;
+      var sd : Sdata2;
+      var k : Key;
+      if (in_dom i mCompleted && in_dom i mStarted && in_dom i mEexp) {
+        sd = proj mStarted.[i];
+        k = h2(gen_sstring (proj mEexp.[i]) (proj mSk.[sd2_actor sd])
+                           (sd2_peer sd) (proj mCompleted.[i])
+                           (sd2_role sd));
+        r = Some k;
+      }
+      return r;
+    }
+
+    fun sessionRev(i : Sidx) : Key option = {
+      var r : Key option = None;
+      if (in_dom i mCompleted && in_dom i mStarted && in_dom i mEexp) {
+        evs = SessionRev(compute_sid mStarted mEexp mCompleted i)::evs;
+        r = computeKey(i);
+      }
+      return r;
+    }
+  }
+  
+  module A = FA(O)
+
+  fun main() : bool = {
+    var b : bool = def;
+    var pks : Pk list = [];
+    var t_idx : Sidx = def;
+    var key : Key = def;
+    var keyo : Key option = def;
+    var b' : bool = def;
+    var i : int = 0;
+    var sidxs : Sidx set = univ_Sidx;
+    var sidx : Sidx = def;
+    var ska : Sk = def;
+    var pka : Pk = def;
+
+    init();
+    while (i < qAgent) {
+      i = i + 1;
+      ska = $sample_Sk;
+      pka = gen_pk(ska);
+      pks = pka :: pks;
+      mSk.[pka] = ska;
+    }
+
+    while (sidxs <> FSet.empty) {
+      sidx = pick sidxs;
+      sidxs = rm sidx sidxs;
+      mEsk.[sidx] = $sample_Esk;
+    } 
+
+    t_idx = A.choose(pks);
+    b = ${0,1};
+    if (in_dom t_idx mStarted && in_dom t_idx mCompleted && in_dom t_idx mEexp) {
+      test = Some (compute_sid mStarted mEexp mCompleted t_idx);
+        (* the if-condition implies "mem (Accept (proj O.test)) O.evs" *)
+      if (b) {
+        keyo = O.computeKey(t_idx);
+      } else {
+        key  = $sample_Key;
+        keyo = Some key;
+      }
+      b' = A.guess(keyo);
+    }
+    return (b = b');
+  }
+}.
+
+local
+lemma Eq_AKE_1_AKE_2:
+  equiv[ AKE_1(A).main ~ AKE_2(A).main : true ==>
+            (res /\ test_fresh AKE_1.test AKE_1.evs){1}
+         => (res /\ test_fresh AKE_2.test AKE_2.evs){2} ].
+proof strict.
+  admit. (* Lazy to eager random oracle *)
+qed.
+
+op bad_esk_col_op : (Sidx, Esk) map -> bool.
+
+op sidx_to_int: Sidx -> int.
+axiom sidx_to_int_inj(i : Sidx) (j : Sidx):
+  sidx_to_int i = sidx_to_int j => i = j.
+
+axiom bad_esk_col_op_def(mEsk : (Sidx, Esk) map):
+    bad_esk_col_op mEsk =
+    (exists i j,    sidx_to_int i < sidx_to_int j
+                 /\ mEsk.[i] <> None /\ mEsk.[i] = mEsk.[j]).
+
+op bad_esk_norev_op : (Sidx, Esk) map -> (Sidx, Sdata2) map
+     -> (Sidx, Eexp) map -> Esk -> Event list -> bool.
+
+axiom bad_esk_norev_op_def(mEsk : (Sidx, Esk) map)
+                          (mStarted : (Sidx, Sdata2) map)
+                          (mEexp : (Sidx, Eexp) map)
+                          (x : Esk)
+                          (evs : Event list):
+  bad_esk_norev_op mEsk mStarted mEexp x evs =
+  (exists i,
+     mEsk.[i] = Some x /\
+     ! (mem (EphemeralRev (compute_psid mStarted mEexp i)) evs)).
+
+(* Add bad flags bad_esk_col and bad_esk_guess *)
+local
 module AKE_3(FA : Adv) = {
   
   var evs  : Event list               (* events for queries performed by adversary *)
@@ -1834,12 +1570,11 @@ module AKE_3(FA : Adv) = {
   var mStarted   : (Sidx, Sdata2) map (* map of started sessions *)
   var mCompleted : (Sidx, Epk)   map  (* additional data for completed sessions *)
 
-  var bad_esk_col : bool              (* esk collision with dom(mH1) *)
-    (* The esk sampled in init1/resp is already in dom(mH1). Since
-       dom(mH1) = sH1 u <earlier esks>, this corresponds to
-       esk-earlier-esk collisions and esk-earlier-h1_a collisions *)
+  var bad_esk_col : bool              (* esk collision *)
+    (* There are two session indexes with the same ephemeral key. *)
 
   var bad_esk_norev : bool            (* h1_a query without previous reveal *)
+    (* There is a h1_a(x,_) query such that Ex i. mEsk[i] = Some x and no EphemeralRev for i *)
 
   fun init() : unit = {
     evs = [];
@@ -1873,13 +1608,10 @@ module AKE_3(FA : Adv) = {
     fun h1_a(a : Sk, x : Esk) : Eexp option = {
       var r : Eexp option = None;
       var xe : Eexp;
+      if (bad_esk_norev_op mEsk mStarted mEexp x evs)
+        bad_esk_norev = true;
       if (cH1 < qH1) {
         cH1 = cH1 + 1;
-        if (any (lambda i, proj mEsk.[i] = x /\
-                           ! (mem (EphemeralRev (compute_psid mStarted mEexp i)) evs))
-                (fdom mStarted)) {
-          bad_esk_norev = true;
-        }
         sH1 = add (a,x) sH1;
         xe = h1(a,x);
         r = Some(xe);
@@ -1914,7 +1646,6 @@ module AKE_3(FA : Adv) = {
       var r : Epk option = None; 
       if (in_dom A mSk && in_dom B mSk && !in_dom i mStarted) {
         x = proj mEsk.[i];
-        if (mem x (queried_esks mH1)) bad_esk_col = true;
         mEexp.[i] = h1(proj (mSk.[A]),x);
         pX = gen_epk(proj mEexp.[i]);
         mStarted.[i] = (A,B,init);
@@ -1930,7 +1661,6 @@ module AKE_3(FA : Adv) = {
       var r : Epk option = None; 
       if (in_dom A mSk && in_dom B mSk && !in_dom i mStarted && !in_dom i mCompleted) {
         y = proj mEsk.[i];
-        if (mem y (queried_esks mH1)) bad_esk_col = true;
         mEexp.[i] = h1(proj (mSk.[B]),y);
         pY = gen_epk(proj mEexp.[i]);
         mStarted.[i] = (B,A,resp);
@@ -2001,12 +1731,13 @@ module AKE_3(FA : Adv) = {
     var b' : bool = def;
     var i : int = 0;
     var sidxs : Sidx set = univ_Sidx;
-    var sidx : Sidx;
+    var sidx : Sidx = def;
     var ska : Sk = def;
     var pka : Pk = def;
 
     init();
     while (i < qAgent) {
+      i = i + 1;
       ska = $sample_Sk;
       pka = gen_pk(ska);
       pks = pka :: pks;
@@ -2019,6 +1750,8 @@ module AKE_3(FA : Adv) = {
       mEsk.[sidx] = $sample_Esk;
     } 
 
+    if (bad_esk_col_op mEsk) bad_esk_col = true;
+    
     t_idx = A.choose(pks);
     b = ${0,1};
     if (in_dom t_idx mStarted && in_dom t_idx mCompleted && in_dom t_idx mEexp) {
@@ -2036,28 +1769,470 @@ module AKE_3(FA : Adv) = {
   }
 }.
 
-lemma Eq_AKE_2_AKE_3(A <: Adv{AKE_2, AKE_3}):
+local
+lemma Eq_AKE_2_AKE_3:
   equiv[ AKE_2(A).main ~ AKE_3(A).main : true ==>
-            (res /\ test_fresh AKE_2.test AKE_2.evs /\
-             !AKE_2.bad_esk_col /\ !AKE_2.bad_esk_norev){1}
-         => (res /\ test_fresh AKE_3.test AKE_3.evs /\
-             !AKE_3.bad_esk_col /\ !AKE_3.bad_esk_norev){2} ].
+            (res /\ test_fresh AKE_2.test AKE_2.evs){1}
+         => (res /\ test_fresh AKE_3.test AKE_3.evs){2} ].
 proof strict.
-  admit. (* Lazy to eager random oracle *)
+  admit. (* We just added some ghost state and ghost code for setting bad. *)
 qed.
 
-(* Do not query h1 in init1 and resp, instead sample Eexp and store
-   it in mEexp (as before).
-   For queries h1_a(a,x), check if there is i such that
-     x = proj mEexp.[i] /\ proj mSk.[sd2_actor (proj mStarted.[i])].
-   If yes, take this value.
-   Invariant:
-   .. disjoint mH1{2} and mEexp ..
-   forall x a x',
-     mH1{1}.[(x,a)] = Some x' <=>
-     (mH1{2}.[(x,a)] = Some x' \/
-      exists i, .. see above ..)
-*)
+(*{ Proof: Bound probability of bad_esk_col *)
+
+op bad_esk_col_x_op : (Sidx, Esk) map -> Esk -> bool.
+
+axiom bad_esk_col_x_op_def(mEsk : (Sidx, Esk) map) (x : Esk):
+  bad_esk_col_x_op mEsk x = (exists i, mEsk.[i] = Some x).
+
+(* Minimal game to bound probability *)
+local
+module AKE_3_1(FA : Adv) = {
+  var mEsk : (Sidx, Esk) map    (* map for ephemeral secret keys *)
+
+  fun main() : bool = {
+    var sidxs : Sidx set = univ_Sidx;
+    var sidx : Sidx = def;
+    var x : Esk = def;
+    var bad_esk_col : bool = false;
+ 
+    mEsk = Map.empty;
+
+    while (sidxs <> FSet.empty) {
+      sidx = pick sidxs;
+      sidxs = rm sidx sidxs;
+      x = $sample_Esk;
+      if (bad_esk_col_x_op mEsk x) bad_esk_col = true;
+      mEsk.[sidx] = x;
+    }
+
+    return bad_esk_col;
+  }
+}.
+
+lemma bad_esk_col_x_op_imp_bad_esk_col_op(mEsk : (Sidx, Esk) map) (i : Sidx) (x : Esk) :
+  mEsk.[i] = None => bad_esk_col_x_op mEsk x => bad_esk_col_op mEsk.[i <- x].
+proof strict.
+  intros=> H_i_none.
+  rewrite !bad_esk_col_op_def bad_esk_col_x_op_def.
+  intros=> Hex; elim Hex; intros=> i0 Hi0_some.
+  case (sidx_to_int i < sidx_to_int i0). intros=> less.
+    exists i. exists i0. smt.
+  intros=> not_less.
+  exists i0. exists i. smt.
+qed.
+
+lemma not_bad_esk_col_x_imp_not_update(mEsk : (Sidx, Esk) map) (i : Sidx) (x : Esk) :
+  mEsk.[i] = None =>
+  ! bad_esk_col_x_op mEsk x =>
+  bad_esk_col_op mEsk.[i <- x] = bad_esk_col_op mEsk.
+proof strict.
+  intros=> H_i_none.
+  rewrite !bad_esk_col_op_def bad_esk_col_x_op_def.
+  intros=> Hnex.
+  rewrite rw_eq_iff.
+  apply iffI.
+  intros=> Hex; elim Hex; intros a b [Hneq] [Hsome] Heq.
+  case (a = i). intros=> eq_a_i.
+    case (b = i). intros=> eq_b_i.
+       generalize Hsome Heq.
+       rewrite !eq_a_i !eq_b_i !get_setE. smt.
+    intros=> neq_b_i. generalize Hsome Heq. rewrite !eq_a_i !get_setE !get_setNE; smt.
+  intros=> neq_a_i.
+  case (b = i). intros=> eq_b_i.
+    generalize Hsome Heq. rewrite !eq_b_i !get_setE !get_setNE. smt. smt.
+  intros=> neq_b_i. generalize Hsome Heq. rewrite !get_setNE. smt. smt. smt.
+  intros=> Hex; elim Hex; intros a b [Hneq] [Hsome] Heq.
+  case (sidx_to_int a < sidx_to_int b). intros=> less.
+  exists a. exists b. split; first trivial.
+  case (a = i). intros=> eq_a_i.
+    case (b = i). intros=> eq_b_i.
+       rewrite !eq_a_i !eq_b_i !get_setE. smt.
+    intros=> neq_b_i. rewrite !eq_a_i !get_setE !get_setNE; smt.
+  intros=> neq_a_i.
+  case (b = i). intros=> eq_b_i.
+    rewrite !eq_b_i !get_setE !get_setNE. smt. smt.
+  intros=> neq_b_i. rewrite !get_setNE. smt. smt. smt.
+  intros=> nless.
+  exists b. exists a. split; first by smt.
+  case (a = i). intros=> eq_a_i.
+    case (b = i). intros=> eq_b_i.
+       rewrite !eq_a_i !eq_b_i !get_setE. smt.
+    intros=> neq_b_i. rewrite !eq_a_i !get_setE !get_setNE; smt.
+  intros=> neq_a_i.
+  case (b = i). intros=> eq_b_i.
+    rewrite !eq_b_i !get_setE !get_setNE. smt. smt.
+  intros=> neq_b_i. rewrite !get_setNE. smt. smt. smt.
+qed.
+
+local lemma bad_AKE_3_O_h1_a:
+  bd_hoare[ AKE_3(A).O.h1_a : AKE_3.bad_esk_col ==> AKE_3.bad_esk_col] = 1%r.
+proof strict.
+  fun. sp. if. wp. sp. inline AKE_3(A).O.h1. wp. sp. rnd.
+  rewrite -/cpTrue -/(Distr.weight sample_Eexp). smt.
+  skip; smt. skip; smt.
+qed.
+
+local lemma bad_AKE_3_O_h2_a:
+  bd_hoare[ AKE_3(A).O.h2_a : AKE_3.bad_esk_col ==> AKE_3.bad_esk_col] = 1%r.
+proof strict.
+  fun. sp. if. wp. sp. inline AKE_3(A).O.h2. wp. sp. rnd.
+  rewrite -/cpTrue -/(Distr.weight sample_Eexp). smt.
+  skip; smt. skip; smt.
+qed.
+
+local lemma bad_AKE_3_O_init2:
+  bd_hoare[ AKE_3(A).O.init2 : AKE_3.bad_esk_col ==> AKE_3.bad_esk_col] = 1%r.
+proof strict.
+  fun. wp. skip; smt.
+qed.
+
+local lemma bad_AKE_3_O_ephemeralRev:
+  bd_hoare[ AKE_3(A).O.ephemeralRev : AKE_3.bad_esk_col ==> AKE_3.bad_esk_col] = 1%r.
+proof strict.
+  fun. wp. skip; smt.
+qed.
+
+local lemma bad_AKE_3_O_staticRev:
+  bd_hoare[ AKE_3(A).O.staticRev : AKE_3.bad_esk_col ==> AKE_3.bad_esk_col] = 1%r.
+proof strict.
+  fun. wp. skip; smt.
+qed.
+
+local lemma bad_AKE_3_O_sessionRev:
+  bd_hoare[ AKE_3(A).O.sessionRev : AKE_3.bad_esk_col ==> AKE_3.bad_esk_col] = 1%r.
+proof strict.
+  fun. sp. if. inline AKE_3(A).O.computeKey.
+  sp. if. inline AKE_3(A).O.h2. sp. wp. rnd.
+  rewrite -/cpTrue -/(Distr.weight sample_Eexp); smt.
+  skip; smt. wp; skip; smt. skip; smt.
+qed.
+
+local lemma bad_AKE_3_O_init1:
+  bd_hoare[ AKE_3(A).O.init1 : AKE_3.bad_esk_col ==> AKE_3.bad_esk_col] = 1%r.
+proof strict.
+  fun. sp. if. inline AKE_3(A).O.h1. sp. wp. rnd.
+  rewrite -/cpTrue -/(Distr.weight sample_Eexp); smt.
+  skip; smt. wp; skip; smt.
+qed.
+
+local lemma bad_AKE_3_O_resp:
+  bd_hoare[ AKE_3(A).O.resp : AKE_3.bad_esk_col ==> AKE_3.bad_esk_col] = 1%r.
+proof strict.
+  fun. sp. if. inline AKE_3(A).O.h1. sp. wp. rnd.
+  rewrite -/cpTrue -/(Distr.weight sample_Eexp); smt.
+  skip; smt. wp; skip; smt.
+qed.
+
+(* FIXME: we would like to prove that bad_esk_col is preserved *)
+local lemma not_bad_AKE_3_O_h1_a:
+  bd_hoare[ AKE_3(A).O.h1_a : !AKE_3.bad_esk_col ==> !AKE_3.bad_esk_col] = 1%r.
+proof strict.
+  fun. sp. if. wp. sp. inline AKE_3(A).O.h1. wp. sp. rnd.
+  rewrite -/cpTrue -/(Distr.weight sample_Eexp). smt.
+  skip; smt. skip; smt.
+qed.
+
+local lemma not_bad_AKE_3_O_h2_a:
+  bd_hoare[ AKE_3(A).O.h2_a : !AKE_3.bad_esk_col ==> !AKE_3.bad_esk_col] = 1%r.
+proof strict.
+  fun. sp. if. wp. sp. inline AKE_3(A).O.h2. wp. sp. rnd.
+  rewrite -/cpTrue -/(Distr.weight sample_Eexp). smt.
+  skip; smt. skip; smt.
+qed.
+
+local lemma not_bad_AKE_3_O_init2:
+  bd_hoare[ AKE_3(A).O.init2 : !AKE_3.bad_esk_col ==> !AKE_3.bad_esk_col] = 1%r.
+proof strict.
+  fun. wp. skip; smt.
+qed.
+
+local lemma not_bad_AKE_3_O_ephemeralRev:
+  bd_hoare[ AKE_3(A).O.ephemeralRev : !AKE_3.bad_esk_col ==> !AKE_3.bad_esk_col] = 1%r.
+proof strict.
+  fun. wp. skip; smt.
+qed.
+
+local lemma not_bad_AKE_3_O_staticRev:
+  bd_hoare[ AKE_3(A).O.staticRev : !AKE_3.bad_esk_col ==> !AKE_3.bad_esk_col] = 1%r.
+proof strict.
+  fun. wp. skip; smt.
+qed.
+
+local lemma not_bad_AKE_3_O_sessionRev:
+  bd_hoare[ AKE_3(A).O.sessionRev : !AKE_3.bad_esk_col ==> !AKE_3.bad_esk_col] = 1%r.
+proof strict.
+  fun. sp. if. inline AKE_3(A).O.computeKey.
+  sp. if. inline AKE_3(A).O.h2. sp. wp. rnd.
+  rewrite -/cpTrue -/(Distr.weight sample_Eexp); smt.
+  skip; smt. wp; skip; smt. skip; smt.
+qed.
+
+local lemma not_bad_AKE_3_O_init1:
+  bd_hoare[ AKE_3(A).O.init1 : !AKE_3.bad_esk_col ==> !AKE_3.bad_esk_col] = 1%r.
+proof strict.
+  fun. sp. if. inline AKE_3(A).O.h1. sp. wp. rnd.
+  rewrite -/cpTrue -/(Distr.weight sample_Eexp); smt.
+  skip; smt. wp; skip; smt.
+qed.
+
+
+local lemma not_bad_AKE_3_O_resp:
+  bd_hoare[ AKE_3(A).O.resp : !AKE_3.bad_esk_col ==> !AKE_3.bad_esk_col] = 1%r.
+proof strict.
+  fun. sp. if. inline AKE_3(A).O.h1. sp. wp. rnd.
+  rewrite -/cpTrue -/(Distr.weight sample_Eexp); smt.
+  skip; smt. wp; skip; smt.
+qed.
+
+local
+lemma Eq_AKE_3_AKE_3_1_bad_esk_col:
+  equiv[ AKE_3(A).main ~ AKE_3_1(A).main : true ==>
+            AKE_3.bad_esk_col{1} => res{2} ].
+proof strict.
+  fun.
+  seq 12 5:
+    (   ((bad_esk_col_op AKE_3.mEsk){1} = bad_esk_col{2})
+     /\ AKE_3.bad_esk_col{1} = false
+     /\ sidx{1} = sidx{2}
+     /\ sidxs{1} = sidxs{2}
+     /\ AKE_3.mEsk{1} = AKE_3_1.mEsk{2}
+     /\ AKE_3.mEsk{1} = Map.empty
+    ).
+  inline AKE_3(A).init.
+  wp; skip; smt.
+  seq 1 0:
+    (   ((bad_esk_col_op AKE_3.mEsk){1} = bad_esk_col{2})
+     /\ AKE_3.bad_esk_col{1} = false
+     /\ sidx{1} = sidx{2}
+     /\ sidxs{1} = sidxs{2}
+     /\ AKE_3.mEsk{1} = Map.empty
+     /\ AKE_3.mEsk{1} = AKE_3_1.mEsk{2}
+     ).
+  while {1}
+    (   ((bad_esk_col_op AKE_3.mEsk){1} = bad_esk_col{2})
+     /\ AKE_3.bad_esk_col{1} = false
+     /\ sidx{1} = sidx{2}
+     /\ AKE_3.mEsk{1} = Map.empty
+     /\ sidxs{1} = sidxs{2}
+     /\ AKE_3.mEsk{1} = AKE_3_1.mEsk{2}) (qAgent - i{1}).
+    progress.
+    wp.
+    rnd. intros=> &hr. cut H:= lossless_sample_Sk.
+      generalize H. rewrite /Distr.weight => //.
+    wp.
+    skip; smt.
+    skip; smt.
+  seq 1 1:
+    (   ((bad_esk_col_op AKE_3.mEsk){1} = bad_esk_col{2})
+     /\ AKE_3.bad_esk_col{1} = false
+     /\ sidx{1} = sidx{2}
+     /\ sidxs{1} = sidxs{2}
+     /\ AKE_3.mEsk{1} = AKE_3_1.mEsk{2}).
+  while
+    (   ((bad_esk_col_op AKE_3.mEsk){1} = bad_esk_col{2})
+     /\ AKE_3.bad_esk_col{1} = false
+     /\ sidx{1} = sidx{2}
+     /\ sidxs{1} = sidxs{2}
+     /\ (forall i, mem i sidxs{1} => AKE_3.mEsk.[i]{1} = None)
+     /\ AKE_3.mEsk{1} = AKE_3_1.mEsk{2}).
+  wp. rnd. wp.
+  skip. progress. smt.
+    apply eqT. apply bad_esk_col_x_op_imp_bad_esk_col_op. smt. smt. smt.
+    apply not_bad_esk_col_x_imp_not_update. smt. smt. smt.
+  skip. smt.
+  seq 1 0:
+    (   (AKE_3.bad_esk_col{1} = bad_esk_col{2})
+     /\ sidx{1} = sidx{2}
+     /\ sidxs{1} = sidxs{2}
+     /\ AKE_3.mEsk{1} = AKE_3_1.mEsk{2}).
+    wp; skip; smt.
+  seq 1 0 : (AKE_3.bad_esk_col{1} = bad_esk_col{2}).
+  case AKE_3.bad_esk_col{1}.
+    call {1}  (_ : AKE_3.bad_esk_col ==> AKE_3.bad_esk_col).
+      fun (AKE_3.bad_esk_col) => //.
+      by apply A_Lossless_choose.
+      by apply bad_AKE_3_O_h1_a.
+      by apply bad_AKE_3_O_h2_a.
+      by apply bad_AKE_3_O_init1.
+      by apply bad_AKE_3_O_init2.
+      by apply bad_AKE_3_O_resp.
+      by apply bad_AKE_3_O_staticRev.
+      by apply bad_AKE_3_O_ephemeralRev.
+      by apply bad_AKE_3_O_sessionRev.
+      skip; smt.
+  call {1}  (_ : !AKE_3.bad_esk_col ==> !AKE_3.bad_esk_col).
+    fun (!AKE_3.bad_esk_col) => //.
+    by apply A_Lossless_choose.
+    by apply not_bad_AKE_3_O_h1_a.
+    by apply not_bad_AKE_3_O_h2_a.
+    by apply not_bad_AKE_3_O_init1.
+    by apply not_bad_AKE_3_O_init2.
+    by apply not_bad_AKE_3_O_resp.
+    by apply not_bad_AKE_3_O_staticRev.
+    by apply not_bad_AKE_3_O_ephemeralRev.
+    by apply not_bad_AKE_3_O_sessionRev.
+    skip; smt.
+  seq 1 0 : (AKE_3.bad_esk_col{1} = bad_esk_col{2}).
+  by rnd {1}; skip; smt.
+  if {1}; [ | by skip; smt ].
+    seq 2 0 : (AKE_3.bad_esk_col{1} = bad_esk_col{2}).
+      sp. if {1}. inline AKE_3(A).O.computeKey. sp. if {1}. wp. inline AKE_3(A).O.h2.
+      sp. wp. rnd {1}. skip. progress.
+      rewrite -/cpTrue -/(Distr.weight sample_Key); smt. wp; skip; smt.
+      wp; rnd {1}. rewrite -/cpTrue -/(Distr.weight sample_Key); skip; smt.
+    case AKE_3.bad_esk_col{1}.
+      call {1}  (_ : AKE_3.bad_esk_col ==> AKE_3.bad_esk_col).
+      fun (AKE_3.bad_esk_col) => //.
+      by apply A_Lossless_guess.
+      by apply bad_AKE_3_O_h1_a.
+      by apply bad_AKE_3_O_h2_a.
+      by apply bad_AKE_3_O_init1.
+      by apply bad_AKE_3_O_init2.
+      by apply bad_AKE_3_O_resp.
+      by apply bad_AKE_3_O_staticRev.
+      by apply bad_AKE_3_O_ephemeralRev.
+      by apply bad_AKE_3_O_sessionRev.
+      skip; smt.
+    call {1}  (_ : !AKE_3.bad_esk_col ==> !AKE_3.bad_esk_col).
+      fun (!AKE_3.bad_esk_col) => //.
+      by apply A_Lossless_guess.
+      by apply not_bad_AKE_3_O_h1_a.
+      by apply not_bad_AKE_3_O_h2_a.
+      by apply not_bad_AKE_3_O_init1.
+      by apply not_bad_AKE_3_O_init2.
+      by apply not_bad_AKE_3_O_resp.
+      by apply not_bad_AKE_3_O_staticRev.
+      by apply not_bad_AKE_3_O_ephemeralRev.
+      by apply not_bad_AKE_3_O_sessionRev.
+      skip; smt.
+qed.
+
+local
+module AKE_3_2(FA : Adv) = {
+  
+  var mEsk : (Sidx, Esk) map    (* map for ephemeral secret keys *)
+
+  fun main() : bool = {
+    var sidxs : Sidx set = univ_Sidx;
+    var sidx : Sidx = def;
+    var x : Esk = def;
+    var bad_esk_col : bool = false;
+    var s1 : Sidx = def;
+    var s2 : Sidx = def;
+ 
+    mEsk = Map.empty;
+
+    while (sidxs <> FSet.empty) {
+      sidx = pick sidxs;
+      sidxs = rm sidx sidxs;
+      x = $sample_Esk;
+      if (bad_esk_col_x_op mEsk x) bad_esk_col = true;
+      mEsk.[sidx] = x;
+    }
+
+    s1 = $sample_Sidx; (* Can we place this directly at the beginning? *)
+    s2 = $sample_Sidx; (* Can we place this directly at the beginning? *)
+    
+    return bad_esk_col;
+  }
+}.
+
+local
+lemma Eq_AKE_3_1_AKE_3_2_bad_esk_col:
+  equiv[ AKE_3_1(A).main ~ AKE_3_2(A).main : true ==> res{1} = res{2} ].
+proof strict.
+  fun.
+  swap {2} 5 3.
+  swap {2} 5 2.
+  seq 6 6 :   (bad_esk_col{1} = bad_esk_col{2}).
+  eqobs_in.
+  rnd {2}. rnd {2}. wp. skip; smt.
+qed.
+
+local
+module AKE_3_3(FA : Adv) = {
+  
+  var mEsk : (Sidx, Esk) map    (* map for ephemeral secret keys *)
+
+  fun main() : bool = {
+    var sidxs : Sidx set = univ_Sidx;
+    var sidx : Sidx = def;
+    var x : Esk = def;
+    var bad_esk_col : bool = false;
+    var s1 : Sidx = def;
+    var s2 : Sidx = def;
+ 
+    mEsk = Map.empty;
+
+    s1 = $sample_Sidx;
+    s2 = $sample_Sidx;
+
+    while (sidxs <> FSet.empty) {
+      sidx = pick sidxs;
+      sidxs = rm sidx sidxs;
+      x = $sample_Esk;
+      mEsk.[sidx] = x;
+    }
+    
+    return (sidx_to_int s1 < sidx_to_int s2) &&
+           mEsk.[s1] <> None && mEsk.[s1] = mEsk.[s2];
+  }
+}.
+
+local
+module AKE_3_4(FA : Adv) = {
+  
+  var mEsk : (Sidx, Esk) map    (* map for ephemeral secret keys *)
+
+  fun main() : bool = {
+    var sidxs : Sidx set = univ_Sidx;
+    var sidx : Sidx = def;
+    var x1 : Esk = def;
+    var x2 : Esk = def;
+    var bad_esk_col : bool = false;
+    var s1 : Sidx = def;
+    var s2 : Sidx = def;
+ 
+    mEsk = Map.empty;
+
+    s1 = $sample_Sidx;
+    s2 = $sample_Sidx;
+
+    x1 = $sample_Esk;
+    x2 = $sample_Esk;
+    
+    return (sidx_to_int s1 < sidx_to_int s2) && x1 = x2;
+  }
+}.
+
+(* sample mEsk.[s1] first, then sample mEsk.[s2] *)
+local
+lemma Eq_AKE_3_3_AKE_3_4_bad_esk_col:
+  equiv[ AKE_3_3(A).main ~ AKE_3_4(A).main : true ==> res{1} = res{2} ].
+proof strict.
+  fun.
+  seq 9 9 : (={s1,s2}). admit.
+  splitwhile (pick sidxs <> s1 /\ pick sidxs <> s2) : {1} 1.
+  unroll {1} 2.
+  swap {2} 9 1.
+  swap {2} 8 1.
+  eqobs_in.
+qed.
+
+local
+lemma Eq_AKE_3_2_AKE_3_3_bad_esk_col:
+  bd_hoare[ AKE_3_3(A).main : true ==>  mEsk.[s] = x] < 1/2%r.
+proof strict.
+  fun.
+  swap {2} 7 1.
+  eqobs_in.
+qed.
+
+
+(*{ end: Proof: Bound probability of bad_esk_col *)
+
+(* Split mH1 into mEexp and mH1A. *)
 module AKE_4(FA : Adv) = {
   
   var evs  : Event list               (* events for queries performed by adversary *)
@@ -2065,8 +2240,8 @@ module AKE_4(FA : Adv) = {
 
   var cH1, cH2 : int                  (* counters for queries *)
 
-  var mH1 : ((Sk * Esk), Eexp) map    (* map for h1 *)
-  var sH1 : (Sk * Esk) set            (* adversary queries for h1 *)
+  var mH1A : ((Sk * Esk), Eexp) map   (* map for h1_a *)
+  var sH1  : (Sk * Esk) set           (* adversary queries for h1 *)
 
   var mH2 : (Sstring, Key) map        (* map for h2 *)
   var sH2 : Sstring set               (* adversary queries for h2 *)
@@ -2077,12 +2252,11 @@ module AKE_4(FA : Adv) = {
   var mStarted   : (Sidx, Sdata2) map (* map of started sessions *)
   var mCompleted : (Sidx, Epk)   map  (* additional data for completed sessions *)
 
-  var bad_esk_col : bool              (* esk collision with dom(mH1) *)
-    (* The esk sampled in init1/resp is already in dom(mH1). Since
-       dom(mH1) = sH1 u <earlier esks>, this corresponds to
-       esk-earlier-esk collisions and esk-earlier-h1_a collisions *)
+  var bad_esk_col : bool              (* esk collision *)
+    (* There are two session indexes with the same ephemeral key. *)
 
   var bad_esk_norev : bool            (* h1_a query without previous reveal *)
+    (* There is a h1_a(x,_) query such that Ex i. mEsk[i] = Some x and no EphemeralRev for i *)
 
   fun init() : unit = {
     evs = [];
@@ -2116,13 +2290,11 @@ module AKE_4(FA : Adv) = {
     fun h1_a(a : Sk, x : Esk) : Eexp option = {
       var r : Eexp option = None;
       var xe : Eexp;
+      if (bad_esk_norev_op mEsk mStarted mEexp x evs)
+        bad_esk_norev = true;
+      (* modify here *)
       if (cH1 < qH1) {
         cH1 = cH1 + 1;
-        if (any (lambda i, proj mEsk.[i] = x /\
-                           ! (mem (EphemeralRev (compute_psid mStarted mEexp i)) evs))
-                (fdom mStarted)) {
-          bad_esk_norev = true;
-        }
         sH1 = add (a,x) sH1;
         xe = h1(a,x);
         r = Some(xe);
@@ -2157,7 +2329,7 @@ module AKE_4(FA : Adv) = {
       var r : Epk option = None; 
       if (in_dom A mSk && in_dom B mSk && !in_dom i mStarted) {
         x = proj mEsk.[i];
-        if (mem x (queried_esks mH1)) bad_esk_col = true;
+        (* modify here *)
         mEexp.[i] = h1(proj (mSk.[A]),x);
         pX = gen_epk(proj mEexp.[i]);
         mStarted.[i] = (A,B,init);
@@ -2173,7 +2345,7 @@ module AKE_4(FA : Adv) = {
       var r : Epk option = None; 
       if (in_dom A mSk && in_dom B mSk && !in_dom i mStarted && !in_dom i mCompleted) {
         y = proj mEsk.[i];
-        if (mem y (queried_esks mH1)) bad_esk_col = true;
+        (* modify here *)
         mEexp.[i] = h1(proj (mSk.[B]),y);
         pY = gen_epk(proj mEexp.[i]);
         mStarted.[i] = (B,A,resp);
@@ -2244,12 +2416,13 @@ module AKE_4(FA : Adv) = {
     var b' : bool = def;
     var i : int = 0;
     var sidxs : Sidx set = univ_Sidx;
-    var sidx : Sidx;
+    var sidx : Sidx = def;
     var ska : Sk = def;
     var pka : Pk = def;
 
     init();
     while (i < qAgent) {
+      i = i + 1;
       ska = $sample_Sk;
       pka = gen_pk(ska);
       pks = pka :: pks;
@@ -2262,6 +2435,8 @@ module AKE_4(FA : Adv) = {
       mEsk.[sidx] = $sample_Esk;
     } 
 
+    if (bad_esk_col_op mEsk) bad_esk_col = true;
+    
     t_idx = A.choose(pks);
     b = ${0,1};
     if (in_dom t_idx mStarted && in_dom t_idx mCompleted && in_dom t_idx mEexp) {
@@ -2278,16 +2453,6 @@ module AKE_4(FA : Adv) = {
     return (b = b');
   }
 }.
-
-lemma Eq_AKE_2_AKE_3(A <: Adv{AKE_2, AKE_3}):
-  equiv[ AKE_2(A).main ~ AKE_3(A).main : true ==>
-            (res /\ test_fresh AKE_2.test AKE_2.evs /\
-             !AKE_2.bad_esk_col /\ !AKE_2.bad_esk_norev){1}
-         => (res /\ test_fresh AKE_3.test AKE_3.evs /\
-             !AKE_3.bad_esk_col /\ !AKE_3.bad_esk_norev){2} ].
-proof strict.
-  admit. (* Use Interval type for domain. Lazy to eager random oracle *)
-qed.
 
 lemma Pr_AKE_1_bad(A <: Adv) &m:
        Pr[ AKE_1(A).main() @ &m : res /\ test_fresh AKE_1.test AKE_1.evs ]
